src/Lib/BCT/BFL/Exec.v
@@ -1,0 +1,37 @@
+Require Import Core.Core Core.Notations Types.
+
+Fixpoint aux_loop (ptr : list Z) (len len_r skip oct size sizeofval : Z)
+  : (Z * Z * Z * Z) := 
+  match ptr with
+  | x :: xs => if (negb (oct =? 0)) && ((skip + 1) <=? size)
+              then if (len >> ((8 * sizeofval) - (8 + 1))) =? 0
+                   then let len' := (len << 8) or x in
+                        aux_loop xs len' len_r (skip + 1) (oct - 1) size sizeofval
+                   else (-1, oct, len, skip)
+              else (0, oct, len, skip)
+  | nil => (0, 0, 0, 0)
+  end.
+
+Definition bfl_loop (ptr : list Z) (len len_r skip oct size sizeofval : Z) 
+  := aux_loop ptr len len_r skip oct size sizeofval.
+
+Definition ber_fetch_len (ptr : list Z) (isc len_r size sizeofval rssizem : Z) 
+  : (Z * Z) :=
+  if size =? 0
+  then (0, len_r)
+  else let oct := hd 0 ptr in 
+       if (oct & 128) =? 0
+       then (1, oct)
+       else if (negb (isc =? 0)) && (oct =? 128) 
+            then (1, -1)
+            else if oct =? 255
+                 then (-1, len_r)
+                 else let oct := oct & 127 in
+                      match bfl_loop (skipn 1%nat ptr) 0 len_r 1 oct size sizeofval with
+                      | (-1, _, _, _) => (-1, len_r)
+                      | (_, oct, len, skip) => if oct =? 0 
+                                              then if (len <? 0) || (len >? rssizem)
+                                                   then (-1, len_r)
+                                                   else (skip, len)
+                                              else (0, len_r)
+                      end.
