src/Lib/BCT/BFL/Vst.v
@@ -1,0 +1,228 @@
+Require Import Core.Core Core.StructNormalizer VstLib.
+Require Import VST.floyd.proofauto.
+(* Require Import BFL.Exec. *)
+Require Import Clight.ber_tlv_length.
+Require Import Core.Notations Core.SepLemmas Core.Tactics Core.VstTactics.
+
+Instance CompSpecs : compspecs. Proof. make_compspecs prog. Defined.
+Definition Vprog : varspecs. Proof. mk_varspecs prog. Defined.
+
+Section Ber_fetch_len.
+
+Open Scope  bool.
+Open Scope int.
+Fixpoint aux_loop ptr len skip oct size sizeofval :
+   (int * int * int * int) := 
+  match ptr with
+  | x :: xs => if (negb (oct == 0)) && ((skip + 1) <=u size)
+              then if (len >> ((Int.repr 8 * sizeofval) - (Int.repr 8 + 1))) == 0
+                   then let len' := Int.or (len << Int.repr 8) x in
+                        aux_loop xs len' (skip + 1) (oct - 1) size sizeofval
+                   else (Int.neg 1, oct, len, skip)
+              else (0, oct, len, skip)
+  | nil => (0, 0, 0, 0)
+  end.
+
+Definition bfl_loop ptr len  skip oct size sizeofval
+  := aux_loop ptr len skip oct size sizeofval.
+
+
+Definition ber_fetch_len ptr isc len_r size sizeofval rssizem : 
+   (int * int) :=
+  if eq_dec size 0
+  then (0, len_r)
+  else let oct := Znth 0 ptr in 
+       if eq_dec (oct & Int.repr 128) 0
+       then (1, oct)
+       else if (negb (isc =? 0)) && (oct == Int.repr 128) 
+            then (1, Int.neg 1)
+            else if eq_dec oct (Int.repr 255)
+                 then (Int.neg 1, len_r)
+                 else let oct := oct & (Int.repr 127) in
+                      match bfl_loop (skipn 1%nat ptr) 0 1 oct size sizeofval with
+                      | (z, oct, len, skip) => if eq_dec z (Int.neg 1) 
+                                       then (z, len_r)
+                                       else 
+                                         if eq_dec oct 0 
+                                              then if (len < 0) || (rssizem < len)
+                                                   then (Int.neg 1, len_r)
+                                                   else (skip, len)
+                                              else (0, len_r)
+                      end.
+Open Scope Z.
+
+Definition ber_fetch_len_spec : ident * funspec :=
+  DECLARE _ber_fetch_length
+    WITH c : Z,  b : block, i : ptrofs,
+         size : int, data : list int,
+         len_r : val
+    PRE [tint, tptr tvoid, tuint, tptr tint]
+      PROP ((* definite length *)
+           (Znth 0 data & Int.repr 128)%int = 0%int;
+             (* primitive tag *)
+            c = 0;
+            Ptrofs.unsigned i + len data < Ptrofs.modulus;
+            Forall (fun x => 0 <= Int.unsigned x <= Byte.max_unsigned) data;
+            0 < len data)
+      PARAMS (Vint (Int.repr 0); (Vptr b i); Vint size; len_r)
+      GLOBALS ()
+      SEP (data_at Tsh (tarray tuchar (Zlength data)) 
+                   (map Vint data) (Vptr b i);
+           data_at_ Tsh tint len_r)
+    POST [tint]
+      let r := ber_fetch_len data c 0%int size (Int.repr (sizeof tuint))
+       (Int.repr (Int.max_unsigned)) in
+      PROP ()
+      LOCAL (temp ret_temp (Vint ((fst r))))
+      SEP (data_at Tsh (tarray tuchar (Zlength data)) 
+                   (map Vint (data)) (Vptr b i);
+           if eq_dec (fst r) 0%int                     
+           then  data_at_ Tsh tint len_r
+           else if eq_dec (fst r) (Int.neg 1%int)
+                then  data_at_ Tsh tint len_r
+                else 
+                  data_at Tsh tint (Vint (snd r)) len_r).
+
+Definition Gprog := ltac:(with_library prog [ber_fetch_len_spec]).
+
+Lemma Znth_0_cons_sublist :  forall (ls : list int), 
+             0 < len ls ->
+             Znth 0 ls :: sublist 1 (len ls) ls = ls.
+  { intros.
+    erewrite Znth_cons_sublist.
+    autorewrite with sublist.
+    auto. lia. }
+Qed.
+
+Theorem ber_fetch_len_correctness : semax_body Vprog Gprog 
+                                          (normalize_function f_ber_fetch_length
+                                                              composites) 
+                                          ber_fetch_len_spec.
+Proof.
+  start_function.
+  forward.
+  forward_if.
+  forward.
+  assert (data_at Tsh (tarray tuchar (len data)) (map Vint data) (Vptr b i) =
+          (data_at Tsh tuchar (Vint (Znth 0 data)) (Vptr b i) *
+          data_at Tsh (tarray tuchar (len data - 1)) 
+                  (sublist 1 (len data) (map Vint data))
+                  (Vptr b (i + 1)%ptrofs))%logic) as D.
+  { erewrite split_non_empty_list 
+      with (i := Vint (Znth 0 data)) 
+           (j2 := len data - 1) 
+           (ls' := sublist 1 (len data) (map Vint data)).
+    auto. erewrite <- map_sublist;
+            erewrite <- map_cons;
+            f_equal; erewrite Znth_0_cons_sublist; try lia; auto.
+    all: autorewrite with sublist; strip_repr. }
+  erewrite D.
+  Intros.
+  forward.
+  entailer!.
+  eapply Forall_Znth with (i0 := 0) in H2; try lia.
+  forward_if; try contradiction.
+  forward.
+  forward.
+  unfold ber_fetch_len.
+  repeat rewrite_if_b.
+  simpl.
+  erewrite <- D.
+  entailer!.
+Qed.
+
+(* Indefinite length branch:  
+- forward_if (temp _t'1 Vzero); try contradiction.
+  + admit.
+    (* forward.
+       entailer!. *)
+  + forward_if; try contradiction.
+    forward_if.
+    * admit. (* forward.
+      { unfold ber_fetch_len.
+        repeat rewrite_if_b.
+        simpl.
+        entailer!.
+        admit. (* split as before *) } *)
+    * repeat forward.
+      (* Loop *)
+       match goal with
+       | [ _ : _ |-  semax _ ?P ?C ?Post ] =>
+         forward_loop (PROP ( )
+                       LOCAL (temp _skipped (Vint (Int.repr 1));
+                              temp _buf (Vptr b (i + 1)%ptrofs);
+                              temp _len (Vint (Int.repr 0)); 
+                              temp _oct (Vint (Znth 0 data & Int.repr 127)%int);
+                              temp _t'1 Vzero;
+                              temp __is_constructed (Vint (Int.repr 0)); 
+                              temp _bufptr (Vptr b i);
+                              temp _size (Vint size); 
+                              temp _len_r len_r)
+                       SEP (data_at Tsh tuchar (Vint (Znth 0 data)) (Vptr b i);
+                            data_at Tsh (tarray tuchar (len data - 1))
+                                    (sublist 1 (len data) (map Vint data))
+                                    (Vptr b (i + 1)%ptrofs); data_at_ Tsh tint len_r))
+         break: P
+        end.
+       -- (* PRE to LI *) 
+         entailer!.
+       -- (* LI C LI *)
+         forward_if [temp _skipped (if eq_dec (Znth 0 data & Int.repr 127)%int 0%int 
+                                   then Vone
+                                   else (Vint (1 + 1)%int)) ;
+                     temp _t'2 (if eq_dec (Znth 0 data & Int.repr 127)%int 0%int 
+                                then Vzero
+                                else Val.of_bool ((1 + 1)%int <=u size))].
+         ++ repeat forward.
+            repeat rewrite_if_b.
+            entailer!.
+         ++ forward.
+            repeat rewrite_if_b.
+            entailer!.
+         Arguments eq_dec : simpl never.
+         ++ forward_if.
+            ** forward_if; try discriminate.
+               normalize.
+               erewrite split_non_empty_list
+                 with (i := Vint (Znth 1 data))
+                      (j2 := len data - 2)
+                      (ls' := sublist 2 (len data) (map Vint data)).
+               Intros.
+               forward.
+               entailer!.
+               eapply Forall_Znth with (i0 := 1) in H1; try lia.
+               admit. (* 0 <= 1 < len data *)
+               repeat forward.
+               entailer!.
+               1-5: admit.
+            ** forward.
+               entailer!.
+               admit.
+       -- (* BREAK rest POST *)
+         forward_if.
+         forward_if (temp _t'4 (if (0 <? 0)
+                                then Vone 
+                                else (Val.of_bool ((-1) >> 1 >> 1 <? 0)))).
+         ** forward.
+            entailer!.
+         ** forward.
+            entailer!.
+            admit.
+         ** forward_if.
+            --- forward.
+                entailer!.
+                admit.
+                admit.
+            --- forward.
+                forward.
+                entailer!.
+                admit.
+                admit.
+         ** forward.
+            entailer!.
+            admit.
+            admit.
+Admitted.
+*)
+
+End Ber_fetch_len.
