src/Lib/BCT/BFT/Exec.v
@@ -1,0 +1,183 @@
+Require Import Core.Core  Types VST.floyd.proofauto Core.Notations.
+Require Import Core.Tactics.
+
+Open Scope int.
+
+Fixpoint range n :=
+  match n with 
+  | O => []
+  | S m => range m ++ [m]
+  end.
+
+Fixpoint index {A} (f : A -> bool) size ls l :=
+  match ls with
+  | [] => None
+  | x :: tl => 
+    let i := (l - len tl)%Z in
+    if i <=? size 
+    then (if f x then Some i else index f size tl l)
+    else None
+  end.
+
+(* let v := fold_left (append_val data') (range (Z.to_nat j)) 0 in
+                 PROP (v >> Int.repr 23 = 0; *)
+
+Definition append_val ls 
+  := (fun x y =>
+        (x << Int.repr 7) or (Znth (Z.of_nat y) ls & Int.repr 127)). 
+
+Eval cbv in (fold_left (append_val [1;0; Int.repr 2]) [0;1;2]%nat 0).
+Eval cbv in (fold_left (fun x y => ((x << 7) or (Znth (Z.of_nat y) [1;0;2] & 127))%Z
+                                            ) [0;1;2]%nat 0%Z).
+
+
+(*Definition append_val ls 
+  := (fun x y =>
+        if x >> Int.repr 23 == 0 
+        then (x << Int.repr 7) or (Znth (Z.of_nat y) ls & Int.repr 127)
+        else x). *)
+
+Eval cbv in (fold_left ((fun ls x y =>
+        if x >> Int.repr 23 == 0 
+        then (x << Int.repr 7) or (Znth (Z.of_nat y) ls & Int.repr 127)
+        else x) [1]) (range 3%nat) (Int.repr Int.max_unsigned)).
+
+
+Definition bft_loop ls size tclass := 
+  let i := index (fun h => (h & Int.repr 128) == 0) size ls (len ls) in
+  let v := fold_left (append_val ls) (range (Z.to_nat size)) 0 in
+  let r := match i with | Some i => i | None => (size + 1)%Z end in 
+  let ex := existsb (fun n => 
+                let v' := fold_left (append_val ls) (range n) 0 in
+                negb (v' >> Int.repr 23 == 0))
+                    (range (Z.to_nat r)) in
+  if ex then (-1, v) else 
+  match i with
+    | Some i =>
+      let v := fold_left (append_val ls) (range (Z.to_nat i - 1)) 0 in     
+      ((i + 1)%Z, ((v << Int.repr 7) or Znth (i - 1) ls) << Int.repr 2 or tclass)
+    | None => (0%Z, v)
+  end.
+
+Definition ber_fetch_tags (ptr : list int) size   :=
+  if eq_dec size 0%Z
+  then (0%Z, 0)
+  else let val := Znth 0 ptr in 
+       let tclass := val >> Int.repr 6 in 
+       if eq_dec (val & Int.repr 31) (Int.repr 31)
+       then bft_loop (sublist 1 (len ptr) ptr) (size - 1) tclass     
+       else (1%Z, ((val & Int.repr 31) << Int.repr 2) or tclass).
+
+Lemma index_app_gen : forall A (ls1 ls2 ls : list A) f size j,
+                 (size < (j - len ls2) + 1)%Z -> 
+                 index f size ls1 (j - len ls2) = None -> 
+                 index f size (ls1 ++ ls2) j = None. 
+Proof.
+  induction ls1; intros.
+    - induction ls2.
+      + auto.
+      + simpl.
+        replace (j - len ls2 <=? size) with false.
+        auto.
+        symmetry.
+        Zbool_to_Prop.
+        autorewrite with sublist in *.
+        list_solve.
+    - intros.
+      simpl in *.
+      break_if; auto.
+      replace (j - len ls2 - len ls1 <=? size) with true in *.
+      break_if.
+      congruence.
+      eapply IHls1.
+      econstructor.
+      lia.
+      auto.
+      symmetry.
+      Zbool_to_Prop.
+      autorewrite with sublist in *.
+      list_solve.
+Qed.
+
+Lemma index_app : forall A (ls1 ls2 ls : list A) f size,
+                 (size < len ls1 + 1)%Z -> 
+                 index f size ls1 (len ls1) = None -> 
+                 index f size (ls1 ++ ls2) (len (ls1 ++ ls2)) = None. 
+Proof.
+  intros.
+  eapply index_app_gen.
+  auto.
+  list_solve.
+  autorewrite with sublist.
+  auto.
+Qed.
+
+Lemma index_spec_Some : forall data1 data2 size b j,
+    (j - len data2 <= size)%Z ->
+    (forall i : Z, 0 <= i < len data1 -> (Znth i data1 & Int.repr 128) <> 0) ->
+    (b & Int.repr 128) = 0 ->
+    index (fun h : int => (h & Int.repr 128) == 0)%int size
+          (data1 ++ (b :: data2)) j 
+    = Some (j - len data2)%Z.
+  { induction data1; intros until j; intros S B Z.
+    - unfold index.
+      cbn -[len].
+      erewrite Z. simpl.
+      break_if.
+      auto.
+      Require Import Core.Tactics.
+      Zbool_to_Prop.
+      lia.
+    - simpl.
+      erewrite IHdata1.
+      replace ((a & Int.repr 128) == 0) with false.
+      break_if.
+      auto.
+      Zbool_to_Prop.
+      autorewrite with sublist in Heqb0.
+      list_solve.
+      symmetry.
+      eapply Int.eq_false.
+      replace a with (Znth 0 (a :: data1)).
+      eapply B.
+      autorewrite with sublist. list_solve.
+      auto.
+      auto.
+      intros.
+      replace (Znth i data1) with (Znth (i + 1) (a :: data1)).
+      eapply B.
+      list_solve.
+      erewrite Znth_pos_cons; try lia.
+      repeat f_equal; lia.
+      eassumption.
+  }
+Qed.
+
+Lemma index_spec_None : forall data size j,
+                 (0 <= len data)%Z ->
+                 (forall i : Z, 0 <= i < len data -> (Znth i data & Int.repr 128) <> 0) ->
+                 index (fun h : int => (h & Int.repr 128) == 0) size 
+                        data j = None.
+  { induction data; intros until j; intros J B.
+    - auto.
+    - simpl.
+      erewrite IHdata.
+      replace ((a & Int.repr 128) == 0) with false.
+      break_if; auto.
+      symmetry.
+      eapply Int.eq_false.
+      replace a with (Znth 0 (a :: data)).
+      eapply B.
+      autorewrite with sublist.
+      list_solve.
+      auto.
+      list_solve.
+      intros. 
+      assert (0 <= i < len (a :: data)) as I.
+      list_solve.
+      replace (Znth i data) with (Znth (i + 1) (a :: data)).
+      eapply B.
+      list_solve.
+      erewrite Znth_pos_cons; try lia.
+      repeat f_equal; lia. }
+Qed.
