src/Lib/BCT/BFT/Vst.v
@@ -1,0 +1,623 @@
+Require Import Core.Core Core.StructNormalizer VstLib.
+Require Import VST.floyd.proofauto.
+ Require Import BFT.Exec. 
+Require Import Clight.ber_tlv_tag.
+Require Import Core.Notations Core.SepLemmas Core.Tactics Core.VstTactics.
+
+Definition Vprog : varspecs. mk_varspecs prog. Defined.
+Instance CompSpecs : compspecs. make_compspecs prog. Defined.
+ 
+Open Scope Z.
+
+Section Ber_fetch_tag.
+
+Definition ber_fetch_tag_spec : ident * funspec :=
+  DECLARE _ber_fetch_tag
+    WITH b : block, i : ptrofs, 
+         data : list int, size : Z, 
+         tag_p : val
+    PRE [tptr tvoid, tuint, tptr tuint]
+      PROP (0 <= size <= Int.max_unsigned;
+            Forall (fun x => 0 <= Int.unsigned x <= Byte.max_unsigned) data;
+            Ptrofs.unsigned i + (Zlength data) < Ptrofs.modulus;
+            0 < len data <= Int.max_unsigned;
+            size < len data)
+      PARAMS ((Vptr b i); Vint (Int.repr size); tag_p)
+      GLOBALS ()
+      SEP (data_at Tsh (tarray tuchar (Zlength data)) 
+                   (map Vint data) (Vptr b i);
+           data_at_ Tsh tuint tag_p)
+    POST [tint]
+      let r := ber_fetch_tags data size in
+      PROP ()
+      LOCAL (temp ret_temp (Vint (Int.repr (fst r))))
+      SEP (data_at Tsh (tarray tuchar (Zlength data)) 
+                   (map Vint data) (Vptr b i);
+           if 0 <? (fst r) 
+           then data_at Tsh tuint (Vint ((snd r))) tag_p
+           else data_at_ Tsh tuint tag_p).
+
+Definition Gprog := ltac:(with_library prog [ber_fetch_tag_spec]).
+
+Lemma Znth_0_cons_sublist :  forall (ls : list int) i, 
+             0 <= i < len ls ->
+             Znth i ls :: sublist (i + 1) (len ls) ls = sublist i (len ls) ls.
+  { intros.
+    erewrite Znth_cons_sublist.
+    autorewrite with sublist.
+    auto. lia. }
+Qed.
+(*
+Theorem ber_fetch_tag : semax_body Vprog Gprog 
+                                   (normalize_function f_ber_fetch_tag composites) 
+                                   ber_fetch_tag_spec.
+Proof.
+  start_function.
+  forward_if.
+  forward.
+  assert (data_at Tsh (tarray tuchar (len data)) (map Vint data) (Vptr b i) =
+          (data_at Tsh tuchar (Vint (Znth 0 data)) (Vptr b i) *
+          data_at Tsh (tarray tuchar (len data - 1)) 
+                  (sublist 1 (len data) (map Vint data))
+                  (Vptr b (i + 1)%ptrofs))%logic) as D.
+  { erewrite split_non_empty_list 
+      with (i := Vint (Znth 0 data)) 
+           (j2 := len data - 1) 
+           (ls' := sublist 1 (len data) (map Vint data)).
+    auto. erewrite <- map_sublist;
+            erewrite <- map_cons;
+            f_equal; erewrite Znth_0_cons_sublist; try lia; auto.
+    all: autorewrite with sublist; strip_repr. }
+  erewrite D.
+  Intros.
+  forward.
+  entailer!.
+  eapply Forall_Znth with (i0 := 0) in H0; try lia.
+  repeat forward.
+  forward_if.
+  repeat forward.
+  erewrite <- D.
+  unfold ber_fetch_tags.
+  repeat rewrite_if_b.
+  simpl.
+  entailer!.
+  repeat forward.
+  (* Loop *)
+  Open Scope int.
+  remember ((Znth 0 data) >> Int.repr 6) as tclass.
+  remember (sublist 1 (len data) data) as data'.
+  match goal with
+  | [ _ : _ |-  semax _ ?P ?C ?Post ] =>
+    forward_loop (
+               EX j : Z, EX v : int, 
+                 let v := fold_left (append_val data') (range (Z.to_nat j)) 0 in
+                 PROP (forall n : nat,
+                          (n < Z.to_nat j)%nat ->
+                          ((fold_left (append_val
+                                         (sublist 1 (len data) data))
+                                      (range n) 0 >> Int.repr 23) == 0) = true;
+                       forall i, (0 <= i < j)%Z -> (Znth i data' & Int.repr 128) <> 0;
+                       0 <= j + 2 <= Int.max_unsigned;
+                       (0 <= j)%Z;
+                       (0 <= j + 1 <= size)%Z)
+                 LOCAL (temp _skipped (Vint (Int.repr (2 + j)));
+                        temp _ptr (Vptr b (i + 1 + Ptrofs.repr j)%ptrofs);
+                        temp _val (Vint v);
+                        temp _t'1 (Vint (Znth 0 data & Int.repr 31)%int);
+                        temp _tclass (Vint (Znth 0 data >> Int.repr 6)%int);
+                        temp _size (Vint (Int.repr size));
+                        temp _tag_r tag_p)
+                 SEP (data_at Tsh tuchar (Vint (Znth 0 data)) (Vptr b i);
+                      data_at Tsh (tarray tuchar j)
+                              (map Vint (sublist 1 (j + 1) data))
+                              (Vptr b (i + 1)%ptrofs);
+                      data_at Tsh (tarray tuchar (len data - j - 1)) 
+                              (map Vint (sublist (j + 1) (len data) data))
+                              (Vptr b (i + 1 + Ptrofs.repr j)%ptrofs);
+                      data_at_ Tsh tuint tag_p))
+            break:            
+             (EX j : Z,
+               let val := fold_left 
+                        (append_val data')
+                              (range (Z.to_nat size - 1)) 0 in
+               PROP (size = (j + 1)%Z;
+                     forall n, (n < Z.to_nat size)%nat 
+                          -> ((fold_left (append_val data')
+                                 (range n) 0
+                                 >> Int.repr 23) == 0) = true;
+                    (index (fun h : int => (h & Int.repr 128) == 0) (size - 1)
+                           (data') (len data') = None)) 
+               LOCAL (temp _skipped (Vint (Int.repr (2 + j)));
+                      temp _ptr (Vptr b (i + Ptrofs.repr j + 1)%ptrofs);
+                      temp _val (Vint val);
+                      temp _t'1 (Vint (Znth 0 data & Int.repr 31)%int);
+                      temp _tclass (Vint (Znth 0 data >> Int.repr 6)%int);
+                      temp _size (Vint (Int.repr size));
+                      temp _tag_r tag_p)
+                 SEP (data_at Tsh tuchar (Vint (Znth 0 data)) (Vptr b i);
+                      data_at Tsh (tarray tuchar (len data - 1)) 
+                              (sublist 1 (len data) (map Vint data))
+                              (Vptr b (i + 1)%ptrofs);
+                      data_at_ Tsh tuint tag_p))
+  end.
+  -- (* PRE to LI *) 
+    Arguments eq_dec : simpl never.
+    Exists 0%Z 0.
+    autorewrite with sublist.
+    entailer!.
+    split.
+    intros.
+    replace n with (Z.to_nat 0).
+    simpl.
+    auto.
+    replace (Z.to_nat 0) with O in * by auto.
+    lia.
+    intro. lia.
+    erewrite data_at_zero_array_eq; auto.
+    repeat erewrite sublist_map.
+    entailer!.
+  -- (* LI C LI *)
+    Intros j v.
+    forward_if.
+    erewrite  Heqdata'.
+    assert (Znth j (sublist 1 (len data) data) =
+                 (Znth (j + 1) data)) as ZNTH.
+    autorewrite with sublist.
+    auto.
+    ++ 
+      assert (data_at Tsh (tarray tuchar (len data - j - 1))
+                      (sublist (j + 1) (len data) (map Vint data))
+                      (Vptr b (i + 1 + Ptrofs.repr j)%ptrofs) =
+              (data_at Tsh tuchar
+                   (Vint (Znth j (sublist 1 (len data) data))) 
+                   (Vptr b (i + 1 + Ptrofs.repr j)%ptrofs) *
+               data_at Tsh (tarray tuchar (len data - j - 2)) 
+                       (sublist (j + 1 + 1) (len data) (map Vint data))
+                       (Vptr b (i + 1 + Ptrofs.repr j + 1)%ptrofs))%logic) as D2.
+  { erewrite split_non_empty_list 
+      with (i := Vint ((Znth j (sublist 1 (len data) data)))) 
+           (j2 := (len data - j - 2)%Z) 
+           (ls' := sublist (j + 1 + 1) (len data) (map Vint data)).
+    auto. repeat erewrite <- map_sublist.
+    erewrite <- map_cons.
+    f_equal. 
+    erewrite ZNTH.
+    erewrite Znth_0_cons_sublist; try lia; auto.
+    
+    all: autorewrite with sublist; strip_repr.
+
+     }
+  replace (Ptrofs.repr 1) with 1%ptrofs by auto with ptrofs.
+  repeat erewrite map_sublist.
+  erewrite D2.
+  Intros.
+  forward.
+  entailer!.
+  eapply Forall_Znth with (i0 := (j + 1)%Z) in H0; autorewrite with sublist; try lia.
+  forward_if.
+  ** forward.
+     forward_if.
+     ---
+     forward.
+     assert (fst (ber_fetch_tags data size) = -1) as F.
+     (* -1 case *)
+     { unfold ber_fetch_tags.
+       repeat rewrite_if_b.
+       clear D.   
+       unfold bft_loop.
+       replace (Z.to_nat (size - 1) + 1)%nat with (Z.to_nat size).
+        assert (range_In : forall n m, (0 <= n < m)%nat -> (0 < m)%nat -> In n (range (m))). 
+         { induction m; intros N M.
+           - lia.
+           - simpl.
+             erewrite in_app.
+             destruct (Nat.eq_dec n (m))%nat.
+             + right.
+               erewrite e.
+               econstructor.
+               auto.
+             + left.
+               eapply IHm; try lia. }
+         assert (existsb
+        (fun n : nat =>
+         negb ((fold_left (append_val (sublist 1 (len data) data)) 
+                       (range n) 0 >> Int.repr 23) == 0))
+        (range (Z.to_nat (size))) = true) as E.
+       { erewrite existsb_exists.
+         exists (Z.to_nat (j + 1)).
+         split.
+        
+       eapply range_In.
+       split.
+       lia.
+       eapply Z2Nat.inj_lt; try lia.
+       replace 0%nat with (Z.to_nat 0).
+       eapply Z2Nat.inj_lt; lia.
+       auto.
+       erewrite negb_true_iff.
+       erewrite Int.eq_false.
+       auto.
+       auto.
+       replace (Z.to_nat (j + 1)) with (S ((Z.to_nat (j)))).
+       simpl.
+       erewrite fold_left_app.
+       simpl.
+       unfold append_val at 1.
+       generalize H13.
+       replace (8 * 4 - 9)%Z with 23 by lia.
+       erewrite Z2Nat.id.
+       auto.
+       lia.
+       erewrite <- Z2Nat.inj_succ.
+       auto.
+       lia. }
+       destruct (index (fun h : int => (h & Int.repr 128) == 0) (size - 1)
+                  (sublist 1 (len data) data) (len (sublist 1 (len data) data))).
+       --  assert (existsb
+        (fun n : nat =>
+         negb ((fold_left (append_val (sublist 1 (len data) data)) 
+                       (range n) 0 >> Int.repr 23) == 0))
+        (range (Z.to_nat z)) = true) as E'.
+       { (* follows from z <= size -1 *) admit. }
+       erewrite E'.
+       auto.
+       --
+       replace (size - 1 + 1)%Z with size by lia.
+       erewrite E.
+       auto.
+       --
+       replace 1%nat with (Z.to_nat 1).
+       erewrite <- Z2Nat.inj_add.
+       f_equal.
+       all: try lia.
+       auto. }
+       rewrite F. 
+       simpl.
+       entailer!.
+     { erewrite sepcon_assoc.
+       erewrite <- D2.
+       erewrite sepcon_assoc.
+       erewrite <- data_at_app_gen.
+       erewrite <- D.
+       entailer!.
+        all: autorewrite with sublist; try lia; auto; strip_repr;
+          try list_solve. }
+     --- (* end the loop *)
+       repeat forward.
+       Exists (j + 1)%Z v.
+       entailer!.
+       repeat split; try lia.
+     { generalize H6 H13.
+    (*   replace ((Z.to_nat (j + 1))) with (S (Z.to_nat j)).
+       simpl.
+       erewrite fold_left_app.
+       simpl.
+       intro.
+       unfold append_val at 1.
+     (*  replace (((Z.of_nat (S (Z.to_nat j)) <=? size)
+      || ((fold_left (append_val data) (range (Z.to_nat j)) 0 >> Int.repr (8 * 4 - 9)) ==
+          0))%bool) with true. *)
+       erewrite Z2Nat.id; try lia.
+       auto.
+       erewrite <- Z2Nat.inj_succ.
+       auto.
+       lia. *) admit. }
+     
+    { intros.
+      destruct (zeq i0 (j)).
+      erewrite e.
+      eassumption.
+      eapply H7.
+      lia. }
+    do 2 f_equal.
+    lia.
+    f_equal.
+    replace ((Z.to_nat (j + 1))) with (S (Z.to_nat j)).
+    simpl.
+    erewrite fold_left_app.
+    cbn -[skipn].
+    unfold append_val at 1.
+   (* replace (Z.of_nat (S (Z.to_nat j)) <=? size) with true.
+    cbn. *)
+    erewrite Z2Nat.id; try lia.
+    auto.
+    erewrite <- Z2Nat.inj_succ.
+    lia.
+    lia.
+ (*   { symmetry.
+      Zbool_to_Prop.
+      generalize H8.
+      strip_repr.
+      erewrite <- Z2Nat.inj_succ.
+      erewrite Z2Nat.id.
+      all: try lia. } *)
+    entailer!.
+    autorewrite with sublist.
+    (* data_at combine proof *) 
+    { erewrite <- ZNTH.
+      erewrite sepcon_assoc.
+      erewrite <- D2.
+      erewrite <- data_at_app_gen.
+      erewrite <- data_at_app_gen.
+      entailer!.
+       all: autorewrite with sublist; try lia; auto; strip_repr;
+          try list_solve.
+       erewrite sublist_map.
+       erewrite <- map_app.
+       f_equal.
+       autorewrite with sublist.
+       auto. }
+  ** (* return skipped case *)
+     repeat forward.
+        
+       remember (((((fold_left (append_val (sublist 1 (len data)  data))) (range (Z.to_nat j))
+                           0 << Int.repr 7) or Znth j (sublist 1 (len data)  data)) <<
+                Int.repr 2) or (Znth 0 data >> Int.repr 6)) as val.
+     assert (ber_fetch_tags data size = (2 + j, val))%Z as RES.
+     { unfold ber_fetch_tags.
+       repeat rewrite_if_b.
+       unfold bft_loop.    
+            
+      assert ((sublist 1 (len data) data) =
+         (sublist 1 (j + 1)%Z data ++
+                      (Znth (j + 1)%Z data ::
+                            sublist (j + 2) (len data) data))) as DT.
+      {  replace (j + 2)%Z with (j + 1 + 1)%Z by lia.
+         erewrite Znth_0_cons_sublist.
+         autorewrite with sublist.
+         auto.
+         lia. }
+      erewrite DT at 1 2.
+      erewrite index_spec_Some.
+      autorewrite with sublist.
+       replace (j +  Z.succ (len data - (j + 2)) - (len data - (j + 2)))%Z
+         with (j + 1)%Z by lia.
+      assert (existsb
+      (fun n : nat =>
+       negb
+         ((fold_left (append_val (sublist 1 (len data) data)) (range n) 0 >> Int.repr 23) == 0))
+      (range (Z.to_nat (j + 1))) = false) as E by admit.
+      erewrite E.
+       erewrite DT at 1 2.
+      erewrite index_spec_Some.
+      autorewrite with sublist.
+       replace (j +  Z.succ (len data - (j + 2)) - (len data - (j + 2)))%Z
+         with (j + 1)%Z by lia.
+       f_equal.
+       lia.
+       subst.
+       assert ((len data - 1 - (len data - (j + 2))) = j + 1)%Z as J.
+       lia.
+       erewrite J.
+        replace (Z.to_nat (j + 1) - 1)%nat with ((Z.to_nat j)).
+      replace (Znth (j + 1) data) with
+          (Znth j (sublist 1 (len data) data)).
+      auto.
+      erewrite Z2Nat.inj_add.
+      replace (Z.to_nat 1) with 1%nat by auto with arith.
+      omega.
+      lia.
+      lia.
+      list_solve.
+      intros.
+      replace (Znth i0 (sublist 1 (j + 1) data)) with 
+          (Znth i0  (sublist 1 (len data) data)).
+      subst.
+      eapply H7.
+      all: try autorewrite with sublist in H25; autorewrite with sublist;
+        auto; try lia.
+      erewrite <- H12.
+      subst.
+      erewrite Znth_sublist; try lia; auto.
+       intros.
+      replace (Znth i0 (sublist 1 (j + 1) data)) with 
+          (Znth i0  (sublist 1 (len data) data)).
+      subst.
+      eapply H7.
+      all: try autorewrite with sublist in H25; autorewrite with sublist;
+        auto; try lia.
+      erewrite <- H12.
+      subst.
+      erewrite Znth_sublist; try lia; auto.
+     
+ }
+      assert (2 + j = fst (ber_fetch_tags data size))%Z as F.
+     { erewrite RES. auto. }
+     assert (0 <? fst (ber_fetch_tags data size) = true) as T
+     by (Zbool_to_Prop; erewrite <- F; lia).
+     erewrite  T.
+     erewrite <- F.
+     remember (sublist 1 (len data) data) as data'.
+     assert (val = snd (ber_fetch_tags data size)) as G.
+     { erewrite RES. auto. }
+     erewrite G.
+     entailer!.
+     (*
+       (data_at Tsh tuchar (Vint (Znth 0 data)) (Vptr b i) *
+   data_at Tsh (tarray tuchar j) (sublist 1 (j + 1) (map Vint data)) (Vptr b (i + 1)%ptrofs) *
+   data_at Tsh (tarray tuchar (len data - j - 1)) (sublist (j + 1) (len data) (map Vint data))
+     (Vptr b (i + Ptrofs.repr j + 1)%ptrofs))%logic
+  |-- data_at Tsh (tarray tuchar (len data)) (map Vint data) (Vptr b i)
+      *)
+     { 
+       erewrite sepcon_comm.
+       erewrite sepcon_comm.
+       erewrite sepcon_assoc.     
+       erewrite sepcon_assoc.
+       erewrite <- D2.
+       replace (i + Ptrofs.repr j + 1)%ptrofs with (((i + 1) + Ptrofs.repr j)%ptrofs).
+       erewrite <- data_at_app_gen.
+       erewrite <- D.
+       entailer!.
+       all: autorewrite with sublist; try lia; auto; try list_solve.
+       strip_repr.
+       strip_repr.
+       f_equal.
+       lia. }
+    ++ (* LI to BREAK *) 
+      forward.
+      Exists j.
+      assert (size = j + 1)%Z by lia.
+      entailer!.
+      replace (Z.to_nat (j + 1) - 1)%nat with (Z.to_nat j).
+      repeat split;
+       try eassumption.
+      admit.
+      replace (sublist 1 (len data) data) with
+          ((sublist 1 (j + 1) data) ++ (sublist (j + 1) (len data) data)).
+      eapply index_app.
+      econstructor.
+      autorewrite with sublist.
+      lia.
+      eapply index_spec_None.
+      list_solve.
+      autorewrite with sublist.
+      intros.
+      replace (Znth i0 (sublist 1 (j + 1) data))
+        with (Znth i0 (sublist 1 (len data) data)).
+      eapply H7; try lia.
+      autorewrite with sublist.
+      auto.
+      autorewrite with sublist.
+      auto.
+      strip_repr.
+      do 2 f_equal.
+      lia.
+      erewrite Z2Nat.inj_add; try lia.
+      replace (Z.to_nat 1) with 1%nat by auto with arith.
+      omega.
+      (* data_at *)
+      { replace (i + Ptrofs.repr (j + 1))%ptrofs with 
+            (i + 1 + Ptrofs.repr j)%ptrofs.
+        erewrite <- data_at_app_gen.
+        entailer!.
+        all: autorewrite with sublist; try lia; auto; try list_solve.
+        erewrite sublist_map.
+        erewrite <- map_app.
+        f_equal.
+        autorewrite with sublist.
+        auto.
+       strip_repr.
+       strip_repr.
+       f_equal.
+       lia.  }
+  --  (* BREAK rest POST *)
+    Intros j.
+    forward.
+    (* return 0 *)
+    assert (0%Z = fst (ber_fetch_tags data (j + 1))) as BF.
+    { unfold ber_fetch_tags.
+      repeat rewrite_if_b.
+      unfold bft_loop.
+      repeat rewrite_if_b.
+      erewrite H8.
+      replace ((j + 1 - 1 + 1))%Z with (j + 1)%Z by lia.
+      assert (existb_forall_false : forall {A} (ls : list A) f, 
+                 (forall a, In a ls -> 
+                       f a = false) ->
+                 existsb f ls = false).
+      { induction ls.
+        - simpl. auto.
+        - intros.
+          simpl.
+          erewrite H6.
+          simpl.
+          eapply IHls.
+          intros.
+          eapply H6.
+          eapply in_cons.
+          auto.
+          econstructor. auto. }                            
+      assert (existsb
+        (fun n : nat =>
+         negb
+           ((fold_left (append_val
+                       (sublist 1 (len data) data)) (range n) 0 >> Int.repr 23) == 0))
+                       (range (Z.to_nat (j))) = false) as G.
+      { replace (Z.to_nat (j + 1) - 1)%nat with (Z.to_nat j) in *.
+        eapply existb_forall_false.
+        intros.
+        erewrite negb_false_iff.
+        eapply H7.
+        assert (range_In_inv : forall m n, In n (range m) -> (n < m)%nat). 
+         { 
+           induction m; intros N M.
+           - contradiction.
+           - simpl in M.
+             erewrite in_app in M.
+             inversion M as [L | R].
+             eapply IHm in L.
+             lia.
+             inversion R.
+             lia.
+             contradiction. } 
+         eapply range_In_inv.
+        (* assert (range_In_monotonicity : 
+                       forall m2 m1 n, (m1 < m2)%nat
+                                  -> In n (range m2) -> In n (range m1)). 
+         { 
+           induction m2; intros until n; intros M I.
+           - contradiction.
+           - simpl in *.
+             erewrite in_app in I.
+             
+             eapply IHm2.
+             lia.
+             destruct (Nat.eq_dec n (S m))%nat.
+             + right.
+               erewrite e.
+               econstructor.
+               auto.
+             + left.
+               eapply IHm; try lia. *)
+           auto.
+        
+    (*   (*  assert (exists x y : Type, x <> y).
+         { exists nat.
+           exists Z. *)
+           replace (Z.to_nat (j + 1)) with (S (Z.to_nat j)).
+             assert (range_In_monotonicity : 
+                       forall n m1 m2, (m1 <= m2)%nat
+                                  -> In n (range m1) -> In n (range m2)). 
+         { 
+           (*induction m; intros N.
+           - simpl.
+             assert (n = 0)%nat as M by lia.
+             erewrite M.
+             lia.
+           - simpl.
+             erewrite in_app.
+             destruct (Nat.eq_dec n (S m))%nat.
+             + right.
+               erewrite e.
+               econstructor.
+               auto.
+             + left.
+               eapply IHm; try lia. *)
+           admit.
+               }
+         eapply range_In_monotonicity with (m1 := Z.to_nat j).
+         lia.
+         auto.
+         admit. (* true as before *) *)
+         admit.
+         replace 1%nat with (Z.to_nat 1).
+         erewrite <- Z2Nat.inj_sub.
+         f_equal.
+         all: try lia.
+         auto. }
+      replace (j + 1 - 1)%Z with j by lia.
+      admit. }
+    admit.
+     (* erewrite G.
+      
+      auto. }
+    erewrite <- BF.
+    simpl.
+    erewrite sepcon_comm.
+    erewrite <- D.
+    entailer!. *)
+Admitted.
+*)
+End Ber_fetch_tag.
+
