src/Lib/BCT/Exec.v
@@ -1,0 +1,104 @@
+Require Import VST.floyd.proofauto.
+Require Import Core.Core Core.Notations Core.Notations Types.
+Require Import ExtLib.Structures.Monad.
+Require Import BFT.Exec BFL.Exec VST.floyd.sublist.
+
+(* assuming ctx is not null *)
+
+Open Scope Z.
+
+Definition ASN__STACK_OVERFLOW_CHECK used_stack max_stack_size := 
+  if eq_dec max_stack_size 0 
+  then 0
+  else if  max_stack_size <? used_stack
+       then -1
+       else 0.
+
+Open Scope bool.
+
+Definition ber_check_tags_primitive ts td ctx size sizeofval sizemax: 
+  option (Z * Z) :=
+  if ASN__STACK_OVERFLOW_CHECK 0 ctx =? 0
+  then let (tag_len, tlv_tag) := ber_fetch_tags ts size  in
+       if (tag_len =? -1) || (tag_len =? 0) then None 
+       else 
+         if (Int.unsigned tlv_tag =? nth O (tags td) 0) 
+         then
+           let (len_len, tlv_len) := ber_fetch_len 
+                                       (sublist 1 (len ts) 
+                                                (map Int.unsigned ts))
+                                                0 0 (size - tag_len) 
+                                                sizeofval sizemax in
+           if (len_len =? -1) || (len_len =? 0) then None 
+           else 
+             let limit_len := tlv_len + tag_len + len_len in
+             if limit_len <? 0 then None
+             else Some (tlv_len, tag_len + len_len)
+         else None
+  else None.
+
+(*
+Parameter ber_fetch_tag : Z -> Z.
+Parameter ber_fetch_length : bool-> Z -> Z.
+Parameter constructed : list Z -> bool.
+Parameter ber_check_tags_loop : Z -> Z -> Z -> option Z.
+
+Open Scope bool.
+
+(* checks the tag, outputs consumed length and expected length *)
+Definition ber_check_tags ts td ctx tag_mode size step : 
+  option Z :=
+  if asn_stack_overflow_check ctx 
+  then Some (-1) 
+  else 
+    let tagno := step + (if tag_mode =? 1 then -1 else 0) in                
+    if (tag_mode =? 0) || (0 <? len (tags td))
+    then 
+      let tag_len := ber_fetch_tag size in
+      if (tag_len =? -1) || (tag_len =? 0) 
+      then None 
+      else let len_len := ber_fetch_length (constructed ts) (size - tag_len) in
+           if (len_len =? -1) || (len_len =? 0) 
+           then None
+           else let size := size - tag_len - len_len in
+                ber_check_tags_loop tagno size step
+    else ber_check_tags_loop tagno size step.
+                 
+(*  
+Theorem ber_check_tags_bool_res : forall td ls,
+    decoder_type td = BOOLEAN_t ->
+    ber_check_tags td ls = Some (mk_check_tag 2 1) 
+    \/ ber_check_tags td ls = None.
+Proof.
+  intros.
+  unfold ber_check_tags; rewrite H.
+  repeat break_match; auto.
+Qed.
+
+Theorem ber_check_tags_bool_Some : forall td ls,
+    decoder_type td = BOOLEAN_t ->
+    ber_check_tags td (Byte.one::Byte.one::ls) = 
+    Some (mk_check_tag 2 1).
+Proof.
+  intros.
+  unfold ber_check_tags.
+  rewrite H.
+  reflexivity.
+Qed.
+
+Theorem ber_check_tags_bool_Some_intro : forall td ls,
+    decoder_type td = BOOLEAN_t ->
+    ber_check_tags td ls = Some (mk_check_tag 2 1) ->
+    exists tl, ls = 1%byte::1%byte::tl.
+Proof.
+  intros td ls DT.
+  unfold ber_check_tags.
+  repeat break_match; try discriminate.
+  intros.
+  unfold andb in Heqb; repeat break_match_hyp; try discriminate.
+  pose proof Byte.eq_spec i 1%byte as T; rewrite Heqb0 in T.
+  pose proof Byte.eq_spec i0 1%byte as T1; rewrite Heqb in T1.
+  rewrite T, T1.
+  exists l0; reflexivity.
+Qed.
+*) *)
