src/Lib/BCT/VST/ASN__STACK_OVERFLOW_CHECK.v
@@ -1,0 +1,88 @@
+Require Import Core.Core Core.StructNormalizer
+        VstLib ErrorWithWriter BCT.Exec.
+Require Import VST.floyd.proofauto Lib.Forward Core.VstTactics.
+Require Import Clight.ber_decoder.
+
+Definition Vprog : varspecs. mk_varspecs prog. Defined.
+Instance CompSpecs : compspecs. make_compspecs prog. Defined.
+
+Definition ASN__STACK_OVERFLOW_CHECK_spec : ident * funspec :=
+  DECLARE _ASN__STACK_OVERFLOW_CHECK
+    WITH ctx_p : val, max_stack_size : Z
+    PRE [tptr (Tstruct _asn_codec_ctx_s noattr)]
+      PROP ()
+      PARAMS (ctx_p)
+      GLOBALS ()
+      SEP (data_at Tsh (Tstruct _asn_codec_ctx_s noattr)
+                   (Vint (Int.repr max_stack_size)) ctx_p)
+    POST [tint]
+      PROP ()
+      LOCAL (temp ret_temp 
+               (Vint
+                  (Int.repr 
+                     (if eq_dec ctx_p nullval 
+                      then 0
+                      else ASN__STACK_OVERFLOW_CHECK 0 max_stack_size ))))
+      SEP (data_at Tsh (Tstruct _asn_codec_ctx_s noattr) 
+                   (Vint (Int.repr max_stack_size)) ctx_p).
+
+Definition Gprog := ltac:(with_library prog [ASN__STACK_OVERFLOW_CHECK_spec]).
+
+Theorem bool_der_encode :
+  semax_body Vprog Gprog 
+             (normalize_function f_ASN__STACK_OVERFLOW_CHECK composites) 
+             ASN__STACK_OVERFLOW_CHECK_spec.
+Proof.
+  (*
+  start_function.
+  repeat forward.
+  forward_if (temp _t'1 (Vint (Int.repr (if eq_dec ctx_p nullval  
+                                         then 0 
+                                         else (if eq_dec max_stack_size 0 
+                                               then 0 
+                                               else 1))))). 
+  - repeat forward.
+    entailer!.
+    unfold isptr in H.
+    destruct ctx_p; try contradiction.
+    unfold nullval.
+    break_if.
+    generalize e. break_if; try congruence.
+    destruct (Int.eq (Int.repr max_stack_size) Int.zero) eqn : N.
+    eapply int_eq_e in N.
+    break_if; auto; try rep_omega.  
+    admit. 
+    eapply int_eq_false_e in N.
+    break_if; auto.
+    erewrite e in *.
+    contradiction.
+  - forward.
+    entailer!.
+  - forward_if True.
+    + forward.
+      forward.
+      entailer!.
+      unfold denote_tc_samebase.
+      admit.
+      forward_if (temp _usedstack 
+                       (force_val (sem_unary_operation Oneg tint 
+                       (force_val (sem_sub_pp tschar ctx_p v_ctx))))).
+      * forward.
+        entailer!.
+        admit.
+        entailer!.
+      * forward.
+        entailer!.
+        admit.
+      * forward.
+        forward.
+        forward_if.
+        entailer!. admit.
+        forward_empty_loop. *)
+Admitted.
+
+    
+
+  
+
+
