src/Lib/BCT/Vst.v
@@ -1,0 +1,1080 @@
+Require Import Core.Core Core.Tactics Core.VstTactics Core.StructNormalizer
+        (* Core.SepLemmas *)
+        VstLib ErrorWithWriter BCT.Exec.
+Require Import VST.floyd.proofauto.
+Require Import Clight.ber_decoder.
+Require Import VST.ASN__STACK_OVERFLOW_CHECK
+    BFT.Vst BFL.Vst   
+ (* ber_fetch_tag ber_fetch_length *) Lib.Forward. 
+Require Import Core.VstTactics Core.Notations.
+Require Import  Clight.ber_decoder.
+
+Definition Vprog : varspecs. mk_varspecs prog. Defined.
+Instance CompSpecs : compspecs. make_compspecs prog. Defined.
+
+Open Scope Z.
+
+Section Ber_check_tags.
+
+Instance Change1 : change_composite_env CompSpecs BFT.Vst.CompSpecs.
+Proof. make_cs_preserve CompSpecs BFT.Vst.CompSpecs. Defined.
+
+Instance Change2 : change_composite_env  BFT.Vst.CompSpecs CompSpecs.
+Proof. make_cs_preserve  BFT.Vst.CompSpecs CompSpecs. Defined.
+
+Instance Change3 : change_composite_env CompSpecs BFL.Vst.CompSpecs.
+Proof. make_cs_preserve CompSpecs BFL.Vst.CompSpecs. Defined.
+
+Instance Change4 : change_composite_env BFL.Vst.CompSpecs CompSpecs.
+Proof. make_cs_preserve BFL.Vst.CompSpecs CompSpecs. Defined.
+
+Definition ber_check_tags_spec : ident * funspec :=
+  DECLARE _ber_check_tags
+    WITH opt_codec_ctx_p : val, opt_codec_ctx : val,
+         td_p : val, td : TYPE_descriptor, 
+         tags_p : val,
+         opt_ctx_p : val,
+         b : block, i : ptrofs, ptr : list Z,
+         res_p : val,
+         size : Z, tag_mode : Z, last_tag_form : Z,
+         last_length_p : val,
+         opt_tlv_form_p : val,
+         max_stack_size : Z
+    PRE [tptr asn_dec_rval_s, tptr (Tstruct _asn_codec_ctx_s noattr),
+         tptr (Tstruct _asn_TYPE_descriptor_s noattr),
+         tptr (Tstruct _asn_struct_ctx_s noattr), 
+         tptr tvoid, tuint, tint, tint, tptr tint, tptr tint]
+      PROP (tag_mode = 0;
+            last_tag_form = 0;
+            0 < len ptr <= Ptrofs.max_unsigned;
+            (Znth 0 ptr) & 32 = 0;
+            nullval = opt_ctx_p;
+            nullval = opt_tlv_form_p;
+            1 = len (tags td);
+            0 <= Ptrofs.unsigned i + len ptr <= Ptrofs.max_unsigned;
+            Forall (fun x => 0 <= x <= Byte.max_unsigned) ptr;
+            0 <= size <= Int.max_unsigned)
+      PARAMS (res_p; opt_codec_ctx_p; td_p; opt_ctx_p; (Vptr b i); 
+                Vint (Int.repr size);
+                Vint (Int.repr tag_mode); Vint (Int.repr last_tag_form);
+                  last_length_p; opt_tlv_form_p)
+      GLOBALS ((fun _ : ident => Vint 0%int))
+      SEP (data_at Tsh (tarray tuchar (len ptr)) 
+                   (map Vint (map Int.repr ptr)) (Vptr b i);
+           field_at Tsh (Tstruct _asn_TYPE_descriptor_s noattr) 
+                         [StructField _tags] 
+                         tags_p td_p;
+           field_at Tsh (Tstruct _asn_TYPE_descriptor_s noattr) 
+                         [StructField _tags_count] 
+                         (Vint (Int.repr (Zlength (tags td)))) td_p;
+           data_at Tsh (tarray tuint (Zlength (tags td))) 
+                   (map Vint (map Int.repr (tags td))) tags_p;
+           data_at_ Tsh asn_dec_rval_s res_p;
+           data_at_ Tsh tint last_length_p;
+           data_at Tsh (Tstruct _asn_codec_ctx_s noattr) 
+                   (Vint (Int.repr (max_stack_size))) opt_codec_ctx_p)
+    POST [tvoid]
+      PROP ()
+      LOCAL ()
+      SEP (data_at Tsh (tarray tuchar (len ptr)) 
+                   (map Vint (map Int.repr ptr)) (Vptr b i);
+           field_at Tsh (Tstruct _asn_TYPE_descriptor_s noattr) 
+                         [StructField _tags] 
+                         tags_p td_p;
+           field_at Tsh (Tstruct _asn_TYPE_descriptor_s noattr) 
+                         [StructField _tags_count] 
+                         (Vint (Int.repr (Zlength (tags td)))) td_p;
+           data_at Tsh (tarray tuint (Zlength (tags td))) 
+                   (map Vint (map Int.repr (tags td))) tags_p;
+           data_at Tsh (Tstruct _asn_codec_ctx_s noattr) 
+                  (Vint (Int.repr (max_stack_size))) opt_codec_ctx_p;
+        match ber_check_tags_primitive (map Int.repr ptr)
+                                       td max_stack_size
+                              size (sizeof tuint) Int.modulus with
+           | Some v => 
+             data_at Tsh asn_dec_rval_s 
+                     (mk_dec_rval 0 (snd v)) res_p *
+             data_at Tsh tint (Vint (Int.repr (fst v))) last_length_p
+           | None => 
+             data_at Tsh asn_dec_rval_s (mk_dec_rval 2 0) res_p *
+             data_at_ Tsh tint last_length_p
+        end).
+
+Definition assert_spec {cs : compspecs} :=
+   WITH e : bool(* , str2 : val, str3 : val, func : val *)
+   PRE [ (tptr tschar), (tptr tschar), tuint, (tptr tschar)]
+       PROP ()
+       PARAMS (nullval; nullval; Vint (Int.repr 137); nullval) 
+       GLOBALS()
+       SEP ()
+    POST [ tvoid ] 
+       PROP (e = true)
+       LOCAL ()
+       SEP ().
+
+Definition Gprog := ltac:(with_library prog 
+                                       [(___assert_fail, assert_spec);
+                                        ber_check_tags_spec;
+                                        ber_fetch_tag_spec;
+                                        ber_fetch_len_spec;
+                                        ASN__STACK_OVERFLOW_CHECK_spec]).
+(*
+Theorem bool_der_encode : 
+  semax_body Vprog Gprog
+             (normalize_function f_ber_check_tags composites) 
+             ber_check_tags_spec.
+Proof.
+  start_function.
+  subst.
+  repeat forward.
+  forward_if (temp _t'1 Vzero).
+  contradiction.
+  - (* forward.
+    entailer!. *) admit.
+  - forward.
+    forward_call (opt_codec_ctx_p, max_stack_size).
+      assert (-1 <= ASN__STACK_OVERFLOW_CHECK 0 max_stack_size <= 0) as A.
+    { unfold ASN__STACK_OVERFLOW_CHECK.
+      repeat break_if; lia. }
+    forward_if [opt_codec_ctx_p <> nullval;
+                (if eq_dec opt_codec_ctx_p nullval
+                 then 0
+                 else ASN__STACK_OVERFLOW_CHECK 0 max_stack_size) = 0].
+  + admit. (* forward_empty_while.
+  assert (opt_codec_ctx_p <> nullval) as ON.
+  { break_if; try nia.
+    eassumption. }
+  rewrite_if_b. 
+  forward_if True; try contradiction.
+  * (* forward.
+    entailer!. *) admit.
+  * forward_if (temp _t'2 Vzero);
+      try forward; try entailer!.
+    forward_if_add_sep (data_at Tsh (Tstruct _asn_dec_rval_s noattr)
+       (Vint (Int.repr 2), Vint (Int.repr 0)) v_rval) v_rval; 
+      try forward; try entailer!.
+    repeat forward. 
+    assert (ber_check_tags_primitive ptr td max_stack_size
+                            size (sizeof tuint) Int.modulus = None) as N.
+       { unfold ber_check_tags_primitive.
+         assert (ASN__STACK_OVERFLOW_CHECK 0 max_stack_size =? 0 = false) 
+           as AS by (Zbool_to_Prop;
+                    eassumption).
+         erewrite AS.
+         auto. }
+    erewrite N.
+    entailer!.  *)
+  + admit. (* forward.    
+    entailer!.
+    apply repr_inj_signed.
+    repeat break_if; try rep_omega.
+    rep_omega.
+    eassumption. *)
+  + forward_if
+      (temp _t'4 Vzero); try congruence.
+  -- admit. (* forward.
+     entailer!. *)
+  -- forward.
+     forward_if (temp _t'10 
+                  ((force_val
+                  (sem_cast tint tbool
+                  (eval_binop Oeq tint tint
+                    (Vint
+                       (Int.repr 0))
+                    (eval_cast tuint tint (Vint (Int.repr (len (tags td))))))))
+                   )); try discriminate.
+     --- admit. 
+         (* forward.
+         forward.
+         entailer!. *) 
+     ---
+       Arguments eq_dec : simpl never.
+       forward_if True.
+       cbn in H3.
+       unfold sem_cast_i2bool in H3.
+       unfold Val.of_bool in H3.
+       destruct (Int.repr 0 == Int.repr (len (tags td)))%int eqn : S.
+       cbn in H3.
+       eapply int_eq_e in S.
+       erewrite <- H5 in *.
+       discriminate.
+       cbn in H3.
+       setoid_rewrite if_true in H3.
+       discriminate.
+       auto.
+       forward.
+       forward_if True.
+       forward.
+       admit. (* entailer!. *)
+    (*   match goal with
+       | [ _ : _ |-  semax _ (PROPx ?P (LOCALx ?Q (SEPx ?R))) ?C ?Post ] =>
+         replace Q with (gvars (fun x : ident => nullval) :: Q)
+        end. *)
+       (* assert_fail *)
+       forward_call (true).
+       admit. (* entailer!. *)
+       admit. (* entailer!. *)
+     (* MAIN LOOP *)       
+     (* match goal with
+       | [ _ : _ |-  semax _ (PROPx ?P (LOCALx ?Q (SEPx ?R))) ?C ?Post ] =>
+         let Q' := remove_LOCAL _tagno Q in
+         replace Q with Q'
+        end. *)
+       rewrite H0.
+       match goal with
+       | [ _ : _ |-  semax _ (PROPx ?P (LOCALx ?Q (SEPx ?R))) ?C ?Post ] =>
+       (*  let Q' := remove_LOCAL _tagno Q in
+         let Q'' := remove_LOCAL _step Q' in *)
+         forward_loop (
+     EX z : Z,
+     let (tag_len, tlv_tag) := Exec.ber_fetch_tags (map Int.repr ptr)
+                                                   size  in
+     let (len_len, tlv_len) := Exec.ber_fetch_len (sublist 1 (len ptr) ptr) 0 0 
+                                                  (size - tag_len) (sizeof tuint) Int.modulus in
+     let ll := if z =? 0 then -1 else (tlv_len)%Z in (* + tag_len + len_len *)
+     let cm := if z =? 0 then 0 else (tag_len + len_len)%Z in 
+     PROP ( 0 <= z <= 1;
+            if z =? 0 then
+              True else
+           0 < tag_len /\
+           0 < len_len /\
+           0 < tlv_len /\
+           tag_len <> 0 /\
+           len_len <> -1 /\
+           len_len <> 0 /\ 
+           tlv_tag = nth O (tags td) 0)
+     LOCAL (temp _t'10
+              (force_val
+                 (sem_cast tint tbool
+                    (eval_binop Oeq tint tint (Vint (Int.repr 0))
+                       (eval_cast tuint tint (Vint (Int.repr (len (tags td))))))));
+     temp _tagno (Vint (Int.repr z));
+     temp _t'4 Vzero;
+     temp _t'3 (Vint (Int.repr 0));
+     temp _step (Vint (Int.repr z)); 
+     temp _t'1 Vzero; 
+     temp _tlv_constr (Vint (Int.repr (if z =? 0 then -1 else 0)));
+     temp _expect_00_terminators (Vint (Int.repr 0));
+     temp _limit_len (Vint (Int.repr ll)); 
+     temp _consumed_myself (Vint (Int.repr cm));
+     lvar _rval__12 (Tstruct _asn_dec_rval_s noattr) v_rval__12;
+     lvar _rval__11 (Tstruct _asn_dec_rval_s noattr) v_rval__11;
+     lvar _rval__10 (Tstruct _asn_dec_rval_s noattr) v_rval__10;
+     lvar _rval__9 (Tstruct _asn_dec_rval_s noattr) v_rval__9;
+     lvar _rval__8 (Tstruct _asn_dec_rval_s noattr) v_rval__8;
+     lvar _rval__7 (Tstruct _asn_dec_rval_s noattr) v_rval__7;
+     lvar _rval__6 (Tstruct _asn_dec_rval_s noattr) v_rval__6;
+     lvar _rval__5 (Tstruct _asn_dec_rval_s noattr) v_rval__5;
+     lvar _rval__4 (Tstruct _asn_dec_rval_s noattr) v_rval__4;
+     lvar _rval__3 (Tstruct _asn_dec_rval_s noattr) v_rval__3;
+     lvar _rval__2 (Tstruct _asn_dec_rval_s noattr) v_rval__2;
+     lvar _rval__1 (Tstruct _asn_dec_rval_s noattr) v_rval__1;
+     lvar _rval (Tstruct _asn_dec_rval_s noattr) v_rval; 
+     lvar _tlv_len tint v_tlv_len;
+     lvar _tlv_tag tuint v_tlv_tag; 
+     temp __res res_p; temp _opt_codec_ctx opt_codec_ctx_p;
+     temp _td td_p; temp _opt_ctx nullval;
+     temp _ptr (offset_val cm  (Vptr b i));
+     temp _size (Vint (Int.repr (if z =? 0 
+                                 then size - cm
+                                 else if size - tag_len - len_len >? tlv_len
+                                   then tlv_len
+                                   else size - ((tag_len + len_len)%Z))));
+     temp _tag_mode (Vint (Int.repr 0));
+     temp _last_tag_form (Vint (Int.repr 0));
+     temp _last_length last_length_p;
+     temp _opt_tlv_form nullval)
+     SEP (data_at Tsh (Tstruct _asn_codec_ctx_s noattr)
+                  (Vint (Int.repr max_stack_size))
+            opt_codec_ctx_p;
+     data_at_ Tsh (Tstruct _asn_dec_rval_s noattr) v_rval__12;
+     data_at_ Tsh (Tstruct _asn_dec_rval_s noattr) v_rval__11;
+     data_at_ Tsh (Tstruct _asn_dec_rval_s noattr) v_rval__10;
+     data_at_ Tsh (Tstruct _asn_dec_rval_s noattr) v_rval__9;
+     data_at_ Tsh (Tstruct _asn_dec_rval_s noattr) v_rval__8;
+     data_at_ Tsh (Tstruct _asn_dec_rval_s noattr) v_rval__7;
+     data_at_ Tsh (Tstruct _asn_dec_rval_s noattr) v_rval__6;
+     data_at_ Tsh (Tstruct _asn_dec_rval_s noattr) v_rval__5;
+     data_at_ Tsh (Tstruct _asn_dec_rval_s noattr) v_rval__4;
+     data_at_ Tsh (Tstruct _asn_dec_rval_s noattr) v_rval__3;
+     data_at_ Tsh (Tstruct _asn_dec_rval_s noattr) v_rval__2;
+     data_at_ Tsh (Tstruct _asn_dec_rval_s noattr) v_rval__1;
+     data_at_ Tsh (Tstruct _asn_dec_rval_s noattr) v_rval;
+     if z =? 0 then (data_at_ Tsh tint v_tlv_len *
+                     data_at_ Tsh tuint v_tlv_tag)
+     else (data_at Tsh tint (Vint (Int.repr tlv_len)) v_tlv_len *
+                     data_at Tsh tuint (Vint (Int.repr tlv_tag)) v_tlv_tag);
+     data_at Tsh (tarray tuchar (len ptr)) 
+             (map Vint (map Int.repr ptr)) (Vptr b i);
+     field_at Tsh (Tstruct _asn_TYPE_descriptor_s noattr) (DOT _tags) tags_p td_p;
+     field_at Tsh (Tstruct _asn_TYPE_descriptor_s noattr) (DOT _tags_count)
+       (Vint (Int.repr (len (tags td)))) td_p;
+     data_at Tsh (tarray tuint (len (tags td))) 
+             (map Vint (map Int.repr (tags td))) tags_p;
+     data_at_ Tsh asn_dec_rval_s res_p; 
+     data_at_ Tsh tint last_length_p))%assert
+                      (* CONTINUE *)
+                      continue:
+           (let (tag_len, tlv_tag) := Exec.ber_fetch_tags ptr size 0 (sizeof tuint) in
+       let (len_len, tlv_len) :=
+         Exec.ber_fetch_len (sublist 1 (len ptr) ptr) 0 0 (size - tag_len) 
+           (sizeof tuint) Int.modulus in
+       PROP (0 < tag_len;
+           0 < len_len;
+           0 < tlv_len;
+           tag_len <> 0;
+           len_len <> -1;
+           len_len <> 0;
+           tlv_tag = nth O (tags td) 0)
+       LOCAL (temp _t'10
+                (force_val
+                   (sem_cast tint tbool
+                      (eval_binop Oeq tint tint (Vint (Int.repr 0))
+                         (eval_cast tuint tint (Vint (Int.repr (len (tags td))))))));
+       temp _tagno (Vint (Int.repr 0)); temp _t'4 Vzero; temp _t'3 (Vint (Int.repr 0));
+       temp _step (Vint (Int.repr 0)); temp _t'1 Vzero;
+       temp _tlv_constr (Vint (Int.repr (0)));
+       temp _expect_00_terminators (Vint (Int.repr 0));
+       temp _limit_len (Vint (Int.repr ((tlv_len)%Z)));
+       temp _consumed_myself (Vint (Int.repr ((tag_len + len_len)%Z)));
+       lvar _rval__12 (Tstruct _asn_dec_rval_s noattr) v_rval__12;
+       lvar _rval__11 (Tstruct _asn_dec_rval_s noattr) v_rval__11;
+       lvar _rval__10 (Tstruct _asn_dec_rval_s noattr) v_rval__10;
+       lvar _rval__9 (Tstruct _asn_dec_rval_s noattr) v_rval__9;
+       lvar _rval__8 (Tstruct _asn_dec_rval_s noattr) v_rval__8;
+       lvar _rval__7 (Tstruct _asn_dec_rval_s noattr) v_rval__7;
+       lvar _rval__6 (Tstruct _asn_dec_rval_s noattr) v_rval__6;
+       lvar _rval__5 (Tstruct _asn_dec_rval_s noattr) v_rval__5;
+       lvar _rval__4 (Tstruct _asn_dec_rval_s noattr) v_rval__4;
+       lvar _rval__3 (Tstruct _asn_dec_rval_s noattr) v_rval__3;
+       lvar _rval__2 (Tstruct _asn_dec_rval_s noattr) v_rval__2;
+       lvar _rval__1 (Tstruct _asn_dec_rval_s noattr) v_rval__1;
+       lvar _rval (Tstruct _asn_dec_rval_s noattr) v_rval; lvar _tlv_len tint v_tlv_len;
+       lvar _tlv_tag tuint v_tlv_tag; temp __res res_p; temp _opt_codec_ctx opt_codec_ctx_p;
+       temp _td td_p; temp _opt_ctx nullval;
+       temp _ptr (offset_val ((tag_len + len_len)%Z) (Vptr b i));
+       temp _size (Vint (Int.repr (if size - tag_len - len_len >? tlv_len
+                                   then tlv_len
+                                   else size - ((tag_len + len_len)%Z))));
+       temp _tag_mode (Vint (Int.repr 0)); temp _last_tag_form (Vint (Int.repr 0));
+       temp _last_length last_length_p; temp _opt_tlv_form nullval)
+       SEP (data_at Tsh (Tstruct _asn_codec_ctx_s noattr) (Vint (Int.repr max_stack_size))
+              opt_codec_ctx_p; data_at_ Tsh (Tstruct _asn_dec_rval_s noattr) v_rval__12;
+       data_at_ Tsh (Tstruct _asn_dec_rval_s noattr) v_rval__11;
+       data_at_ Tsh (Tstruct _asn_dec_rval_s noattr) v_rval__10;
+       data_at_ Tsh (Tstruct _asn_dec_rval_s noattr) v_rval__9;
+       data_at_ Tsh (Tstruct _asn_dec_rval_s noattr) v_rval__8;
+       data_at_ Tsh (Tstruct _asn_dec_rval_s noattr) v_rval__7;
+       data_at_ Tsh (Tstruct _asn_dec_rval_s noattr) v_rval__6;
+       data_at_ Tsh (Tstruct _asn_dec_rval_s noattr) v_rval__5;
+       data_at_ Tsh (Tstruct _asn_dec_rval_s noattr) v_rval__4;
+       data_at_ Tsh (Tstruct _asn_dec_rval_s noattr) v_rval__3;
+       data_at_ Tsh (Tstruct _asn_dec_rval_s noattr) v_rval__2;
+       data_at_ Tsh (Tstruct _asn_dec_rval_s noattr) v_rval__1;
+       data_at_ Tsh (Tstruct _asn_dec_rval_s noattr) v_rval;
+        data_at Tsh tint (Vint (Int.repr tlv_len)) v_tlv_len ;
+        data_at Tsh tuint (Vint (Int.repr tlv_tag)) v_tlv_tag;
+       data_at Tsh (tarray tuchar (len ptr)) (map Vint (map Int.repr ptr)) (Vptr b i);
+       field_at Tsh (Tstruct _asn_TYPE_descriptor_s noattr) (DOT _tags) tags_p td_p;
+       field_at Tsh (Tstruct _asn_TYPE_descriptor_s noattr) (DOT _tags_count)
+         (Vint (Int.repr (len (tags td)))) td_p;
+       data_at Tsh (tarray tuint (len (tags td))) (map Vint (map Int.repr (tags td))) tags_p;
+       data_at_ Tsh asn_dec_rval_s res_p; data_at_ Tsh tint last_length_p))
+                             break: (
+     let (tag_len, tlv_tag) := Exec.ber_fetch_tags ptr size 0 (sizeof tuint) in
+     let (len_len, tlv_len) := Exec.ber_fetch_len (sublist 1 (len ptr) ptr) 0 0 
+                                                  (size - tag_len) (sizeof tuint) Int.modulus in
+     PROP (0 < tag_len;
+           0 < len_len;
+           0 < tlv_len;
+           tag_len <> 0;
+           len_len <> -1;
+           len_len <> 0;
+           tlv_tag = nth O (tags td) 0)
+     LOCAL (temp _t'10
+              (force_val
+                 (sem_cast tint tbool
+                    (eval_binop Oeq tint tint (Vint (Int.repr 0))
+                       (eval_cast tuint tint (Vint (Int.repr (len (tags td))))))));
+     temp _tagno (Vint (Int.repr 1));
+     temp _t'4 Vzero;
+     temp _t'3 (Vint (Int.repr 0));
+     temp _step (Vint (Int.repr 1)); 
+     temp _t'1 Vzero; 
+     temp _tlv_constr (Vint (Int.repr 0));
+     temp _expect_00_terminators (Vint (Int.repr 0));
+     temp _limit_len (Vint ((Int.repr (tlv_len (* + tag_len + len_len *))))); 
+     temp _consumed_myself (Vint (Int.repr (tag_len + len_len)));
+     lvar _rval__12 (Tstruct _asn_dec_rval_s noattr) v_rval__12;
+     lvar _rval__11 (Tstruct _asn_dec_rval_s noattr) v_rval__11;
+     lvar _rval__10 (Tstruct _asn_dec_rval_s noattr) v_rval__10;
+     lvar _rval__9 (Tstruct _asn_dec_rval_s noattr) v_rval__9;
+     lvar _rval__8 (Tstruct _asn_dec_rval_s noattr) v_rval__8;
+     lvar _rval__7 (Tstruct _asn_dec_rval_s noattr) v_rval__7;
+     lvar _rval__6 (Tstruct _asn_dec_rval_s noattr) v_rval__6;
+     lvar _rval__5 (Tstruct _asn_dec_rval_s noattr) v_rval__5;
+     lvar _rval__4 (Tstruct _asn_dec_rval_s noattr) v_rval__4;
+     lvar _rval__3 (Tstruct _asn_dec_rval_s noattr) v_rval__3;
+     lvar _rval__2 (Tstruct _asn_dec_rval_s noattr) v_rval__2;
+     lvar _rval__1 (Tstruct _asn_dec_rval_s noattr) v_rval__1;
+     lvar _rval (Tstruct _asn_dec_rval_s noattr) v_rval; 
+     lvar _tlv_len tint v_tlv_len;
+     lvar _tlv_tag tuint v_tlv_tag; 
+     temp __res res_p; temp _opt_codec_ctx opt_codec_ctx_p;
+     temp _td td_p; temp _opt_ctx nullval;
+     temp _ptr (offset_val (tag_len + len_len) (Vptr b i));
+     temp _size (Vint (Int.repr ((if size - tag_len - len_len >? tlv_len
+                                  then tlv_len
+                                  else size - ((tag_len + len_len)%Z)))));
+     temp _tag_mode (Vint (Int.repr 0));
+     temp _last_tag_form (Vint (Int.repr 0));
+     temp _last_length last_length_p;
+     temp _opt_tlv_form nullval)
+     SEP (data_at Tsh (Tstruct _asn_codec_ctx_s noattr)
+                  (Vint (Int.repr max_stack_size))
+            opt_codec_ctx_p;
+     data_at_ Tsh (Tstruct _asn_dec_rval_s noattr) v_rval__12;
+     data_at_ Tsh (Tstruct _asn_dec_rval_s noattr) v_rval__11;
+     data_at_ Tsh (Tstruct _asn_dec_rval_s noattr) v_rval__10;
+     data_at_ Tsh (Tstruct _asn_dec_rval_s noattr) v_rval__9;
+     data_at_ Tsh (Tstruct _asn_dec_rval_s noattr) v_rval__8;
+     data_at_ Tsh (Tstruct _asn_dec_rval_s noattr) v_rval__7;
+     data_at_ Tsh (Tstruct _asn_dec_rval_s noattr) v_rval__6;
+     data_at_ Tsh (Tstruct _asn_dec_rval_s noattr) v_rval__5;
+     data_at_ Tsh (Tstruct _asn_dec_rval_s noattr) v_rval__4;
+     data_at_ Tsh (Tstruct _asn_dec_rval_s noattr) v_rval__3;
+     data_at_ Tsh (Tstruct _asn_dec_rval_s noattr) v_rval__2;
+     data_at_ Tsh (Tstruct _asn_dec_rval_s noattr) v_rval__1;
+     data_at_ Tsh (Tstruct _asn_dec_rval_s noattr) v_rval;
+     data_at Tsh tint (Vint (Int.repr tlv_len)) v_tlv_len;
+     data_at Tsh tuint (Vint (Int.repr tlv_tag)) v_tlv_tag;
+     data_at Tsh (tarray tuchar (len ptr)) 
+             (map Vint (map Int.repr ptr)) (Vptr b i);
+     field_at Tsh (Tstruct _asn_TYPE_descriptor_s noattr) (DOT _tags) tags_p td_p;
+     field_at Tsh (Tstruct _asn_TYPE_descriptor_s noattr) (DOT _tags_count)
+       (Vint (Int.repr (len (tags td)))) td_p;
+     data_at Tsh (tarray tuint (len (tags td))) 
+             (map Vint (map Int.repr (tags td))) tags_p;
+     data_at_ Tsh asn_dec_rval_s res_p; 
+     data_at_ Tsh tint last_length_p))
+       end.
+       +++ (* Pre -> LI *)
+        (* Exists 0.
+         repeat rewrite_if_b.
+         repeat break_let.
+         entailer!.
+         apply derives_refl. *) admit.
+       +++ Intros z.
+           repeat break_let.
+           break_if.
+           * simpl.
+             Intros.
+             Zbool_to_Prop.
+             forward.
+           forward_if.
+           2: (* LI -> break *) lia.
+           forward_call (b, i, ptr, size, v_tlv_tag). 
+           { repeat split; try rep_omega.
+             eassumption. }
+           assert (z0 = 65) as Z0 by admit.
+           replace (fst (Exec.ber_fetch_tags ptr size 0 (sizeof tuint)))
+             with z0. (* FIXME : forward switch doesn't work with complex terms *)
+           (* in VST 2.6 forward_switch needs change and can fail here *)
+           match goal with
+           | [ _ : _ |- semax _ ?Pre ?C ?Post ] =>
+             forward_switch Pre
+           end; clear Z0.
+           *** admit. (* (* RC_FAIL  *)             
+              match goal with
+                 | [ _ : _ |- semax _ ?Pre ?C ?Post ] =>
+                   forward_empty_while_break Pre
+              end.
+              assert (opt_codec_ctx_p <> nullval) as ON.
+              { break_if; try nia;
+                eassumption. }
+              rewrite_if_b. 
+              forward_if True; try contradiction.
+              forward.
+              admit. (* entailer!. *) 
+              forward_if (temp _t'12 Vzero);
+               try forward; try entailer!.
+             forward_if_add_sep (data_at Tsh 
+                                         (Tstruct _asn_dec_rval_s noattr)
+                                         (Vint (Int.repr 2), Vint (Int.repr 0))
+                                         v_rval__3) v_rval__3; 
+               try forward; try entailer!.
+             repeat forward. 
+             assert (ber_check_tags_primitive ptr td max_stack_size
+                                              size (sizeof tuint) Int.modulus = None) as N.
+             { unfold ber_check_tags_primitive.
+               erewrite H0.
+               erewrite Heqp.
+               simpl.
+               auto. }
+             erewrite N.
+             (* entailer!. *)
+             admit. *)
+           *** admit. (* (* RC_FAIL: same *)
+              match goal with
+                 | [ _ : _ |- semax _ ?Pre ?C ?Post ] =>
+                   forward_empty_while_break Pre
+              end.
+              assert (opt_codec_ctx_p <> nullval) as ON.
+              { break_if; try nia;
+                eassumption. }
+              rewrite_if_b. 
+              forward_if True; try contradiction.
+              forward.
+              admit. (* entailer!. *) 
+              forward_if (temp _t'12 Vzero);
+               try forward; try entailer!.
+             forward_if_add_sep (data_at Tsh 
+                                         (Tstruct _asn_dec_rval_s noattr)
+                                         (Vint (Int.repr 2), Vint (Int.repr 0))
+                                         v_rval__3) v_rval__3; 
+               try forward; try entailer!.
+             repeat forward. 
+             assert (ber_check_tags_primitive ptr td max_stack_size
+                                              size (sizeof tuint) Int.modulus = None) as N.
+             { unfold ber_check_tags_primitive.
+               erewrite H0.
+               erewrite Heqp.
+               simpl.
+               auto. }
+             erewrite N.
+             (* entailer!. *)
+             admit. *)
+           *** admit. (* forward.
+               entailer!. *) 
+           *** remember (map Vint (map Int.repr ptr)) as ptr'.
+               normalize.
+               Intros. 
+               assert_PROP ((Vptr b i) = 
+                            field_address 
+                              (tarray tuchar (len ptr)) [ArraySubsc 0] (Vptr b i)).
+               { entailer!.
+                 rewrite field_address_offset; cbn.
+                 normalize.
+                 econstructor;
+                 auto.
+                 repeat split; auto; 
+                   autorewrite with norm;  try rep_omega.
+                 cbn.
+                 autorewrite with norm.
+                 rep_omega.
+                 constructor.
+                 intros.
+                 econstructor; auto; cbn.
+                 auto.
+                 eapply Z.divide_1_l. }
+               forward.
+               entailer!.
+               unfold is_int.
+               assert (0 <= Znth 0 ptr <= Byte.max_unsigned) as B.
+               { eapply Forall_Znth.
+                 lia.
+                 eassumption. }
+               repeat erewrite Znth_map; auto; try nia.
+               strip_repr.
+               forward_if (temp _t'13 Vzero).
+             ** admit. 
+                (* assert ((Znth 0 ptr & 32) <> 0) as Z.
+                { generalize H10.
+                  subst.
+                  repeat erewrite Znth_map.
+                  simpl.
+                  autorewrite with norm.
+                  intro V.
+                  eapply typed_true_tint_Vint in V.
+                  eapply repr_neq_e in V.
+                  auto.
+                  lia.
+                  erewrite Zlength_map.
+                  lia. }
+                lia. *)
+             ** admit. (* forward.  entailer!. *)
+             ** forward.
+                forward_if
+                  (temp _t'15 Vzero); try contradiction;
+                  try forward; try entailer!; rewrite_if_b; try entailer!.
+                forward_if True; try nia.
+                forward_if True.
+                forward.
+                admit. (* entailer! *)
+                lia.
+                forward.
+                forward. 
+                normalize.
+                forward.
+                forward_if. 
+             ++ admit. 
+                (* (* RC_FAIL case *) 
+               forward_empty_while.
+              rewrite_if_b. 
+              forward_if True; try contradiction.
+              forward.
+              admit. (* entailer!. *) 
+              forward_if (temp _t'14 Vzero);
+               try forward; try entailer!.
+             forward_if_add_sep (data_at Tsh 
+                                         (Tstruct _asn_dec_rval_s noattr)
+                                         (Vint (Int.repr 2), Vint (Int.repr 0))
+                                         v_rval__4) v_rval__4; 
+               try forward; try entailer!.
+             repeat forward. 
+             assert (ber_check_tags_primitive ptr td max_stack_size
+                                              size (sizeof tuint) Int.modulus = None) as N.
+             { unfold ber_check_tags_primitive.
+               erewrite H0.
+               erewrite Heqp.
+               simpl.
+               assert (z1 <>
+                       (nth 0 (tags td) 0)) as O.
+               { replace z1 with (snd (Exec.ber_fetch_tags ptr size 0 4)).
+                 generalize H11.
+                 erewrite Byte.unsigned_repr.
+                 intro V.
+                 eapply repr_neq_e in V.
+                 easy.
+                 (* lemma: 0 <= snd (Exec.ber_fetch_tags ptr size 0 4)
+                    <= Byte.max_unsigned *)
+                 admit.
+                 cbn in Heqp.
+                 erewrite Heqp.
+                 easy.
+                  }
+               break_if; auto.
+               break_if.
+               Zbool_to_Prop.
+               lia.
+               auto. }
+             erewrite N.
+             admit. (* entailer!. *) *)
+             ++ admit. (* forward. 
+                entailer!. *) 
+             ++  forward.
+                 forward_if True.
+                 lia.
+             ++++ forward_if (temp _t'18 Vzero); try congruence.
+                  forward.
+                  admit. (* entailer!. *)
+                  forward_if.
+                  lia.
+                  forward;  admit. (* entailer!. *) 
+             ++++  
+              (* size : Z, data : list Z,
+                 isc : Z, buf_b : block, buf_ofs : ptrofs,      
+                 res_v : Z, res_ptr : val *)   
+               erewrite Heqptr'.
+               replace (data_at Tsh (tarray tuchar (len ptr))
+                       (map Vint (map Int.repr ptr)) (Vptr b i))
+                       with
+                        (data_at Tsh tuchar (Vubyte (Byte.repr (Znth 0 ptr)))
+                                   (Vptr b i) * 
+                         data_at Tsh (tarray tuchar (len ptr - 1)) 
+                                 (map Vubyte (map Byte.repr (sublist 1 (len ptr) ptr)))
+                                   (Vptr b (i + Ptrofs.repr z0)%ptrofs))%logic.             
+                forward_call (0, Vptr b (i + Ptrofs.repr z0)%ptrofs, size - z0, 
+                             sublist 1 (len ptr) ptr, v_tlv_len).
+                entailer!.
+                cbn.
+                repeat f_equal; auto.
+                strip_repr.
+                (* need Int.min_signed <= z0 <= Int.max_signed *)
+                admit.
+                unfold Frame.
+                instantiate (1 := 
+  [data_at Tsh tuchar (Vubyte (Byte.repr (Znth 0 ptr))) (Vptr b i) *
+   data_at Tsh tuint (Vubyte (Byte.repr 
+                 (snd (Exec.ber_fetch_tags ptr size 0 (sizeof tuint)))))
+     v_tlv_tag *
+   data_at Tsh (Tstruct _asn_codec_ctx_s noattr) (Vint (Int.repr max_stack_size)) 
+           opt_codec_ctx_p *
+   data_at_ Tsh (Tstruct _asn_dec_rval_s noattr) v_rval__12 *
+   data_at_ Tsh (Tstruct _asn_dec_rval_s noattr) v_rval__11 *
+   data_at_ Tsh (Tstruct _asn_dec_rval_s noattr) v_rval__10 *
+   data_at_ Tsh (Tstruct _asn_dec_rval_s noattr) v_rval__9 *
+   data_at_ Tsh (Tstruct _asn_dec_rval_s noattr) v_rval__8 *
+   data_at_ Tsh (Tstruct _asn_dec_rval_s noattr) v_rval__7 *
+   data_at_ Tsh (Tstruct _asn_dec_rval_s noattr) v_rval__6 *
+   data_at_ Tsh (Tstruct _asn_dec_rval_s noattr) v_rval__5 *
+   data_at_ Tsh (Tstruct _asn_dec_rval_s noattr) v_rval__4 *
+   data_at_ Tsh (Tstruct _asn_dec_rval_s noattr) v_rval__3 *
+   data_at_ Tsh (Tstruct _asn_dec_rval_s noattr) v_rval__2 *
+   data_at_ Tsh (Tstruct _asn_dec_rval_s noattr) v_rval__1 *
+   data_at_ Tsh (Tstruct _asn_dec_rval_s noattr) v_rval *
+   field_at Tsh (Tstruct _asn_TYPE_descriptor_s noattr) (DOT _tags) tags_p td_p *
+   field_at Tsh (Tstruct _asn_TYPE_descriptor_s noattr) (DOT _tags_count)
+     (Vint (Int.repr (len (tags td)))) td_p *
+   data_at Tsh (tarray tuint (len (tags td))) (map Vint (map Int.repr (tags td))) tags_p *
+   data_at_ Tsh asn_dec_rval_s res_p * data_at_ Tsh tint last_length_p]%logic).
+                simpl.
+                entailer!.
+                autorewrite with sublist.
+                entailer!.
+                (* need 0 <= size - z0 <= Int.max_unsigned *)
+                admit.
+                Intros v.
+                erewrite H10.
+                assert (z2 = 99) as Z2 by admit.
+                replace (fst
+                       (Exec.ber_fetch_len (sublist 1 (len ptr) ptr) 0 0 
+                          (size - z0) (sizeof tuint) Int.modulus))
+                  with z2.
+                 match goal with
+                 | [ _ : _ |- semax _ ?Pre ?C ?Post ] =>
+                   forward_switch Pre
+                 end. clear Z2.
+             admit. (* (* RC FAIL 
+                 {  match goal with
+                 | [ _ : _ |- semax _ ?Pre ?C ?Post ] =>
+                   forward_empty_while_break Pre
+              end.
+              rewrite_if_b. 
+              forward_if True; try contradiction.
+              forward.
+              admit. (* entailer!. *) 
+              forward_if (temp _t'20 Vzero);
+               try forward; try entailer!.
+             forward_if_add_sep (data_at Tsh 
+                                         (Tstruct _asn_dec_rval_s noattr)
+                                         (Vint (Int.repr 2), Vint (Int.repr 0))
+                                         v_rval__7) v_rval__7; 
+               try forward; try entailer!.
+             repeat forward. 
+             assert (ber_check_tags_primitive ptr td max_stack_size
+                                              size (sizeof tuint) Int.modulus = None) as N.
+             { unfold ber_check_tags_primitive.
+               erewrite H0.
+               erewrite Heqp.
+               erewrite Heqp0.
+               simpl.
+               break_if; auto.
+               break_if; auto.
+               }
+             erewrite N.
+             admit. (* RC_FAIL *) } *) *)
+             admit. (* same *)
+                 forward.
+                 admit. (* entailer! *)
+                 forward.
+                 forward_if.
+                 admit. (* no indefinite length - see ber_fetch_length spec *)
+                 forward_if True; try contradiction.
+                 forward.
+                 admit. (* entailer! *)
+                 forward_if (temp _limit_len
+           (Vint
+              (Int.repr
+                 (Byte.unsigned
+                    (Byte.repr
+                       (snd
+                          (Exec.ber_fetch_len (sublist 1 (len ptr) ptr) 0 0 
+                             (size - z0) (sizeof tuint) Int.modulus)))) + 
+               Int.repr z0 + Int.repr z2)%int)); try contradiction.
+                 forward.
+                 forward.
+                 entailer!.
+                 admit. (* bounds *)
+                 forward_if (temp _limit_len
+           (Vint
+              (Int.repr
+                 (Byte.unsigned
+                    (Byte.repr
+                       (snd
+                          (Exec.ber_fetch_len (sublist 1 (len ptr) ptr) 0 0 
+                             (size - z0) (sizeof tuint) Int.modulus)))) + 
+               Int.repr z0 + Int.repr z2)%int)); try contradiction.
+                 (* RC_FAIL *)
+            admit. (*      {  forward_empty_while.
+              rewrite_if_b. 
+              forward_if True; try contradiction.
+              forward.
+              admit. (* entailer!. *) 
+              forward_if (temp _t'23 Vzero);
+               try forward; try entailer!.
+             forward_if_add_sep (data_at Tsh 
+                                         (Tstruct _asn_dec_rval_s noattr)
+                                         (Vint (Int.repr 2), Vint (Int.repr 0))
+                                         v_rval__10) v_rval__10; 
+               try forward; try entailer!.
+             repeat forward. 
+             assert (ber_check_tags_primitive ptr td max_stack_size
+                                              size (sizeof tuint) Int.modulus = None) as N.
+             { unfold ber_check_tags_primitive.
+               erewrite H0.
+               erewrite Heqp.
+               erewrite Heqp0.
+               simpl.
+               break_if; auto.
+               break_if; auto.
+               generalize H14.
+               strip_repr.
+               erewrite Byte.unsigned_repr.
+               replace (snd (Exec.ber_fetch_len (sublist 1 (len ptr) ptr) 
+                                                0 0 (size - z0) 4 Int.modulus))
+                       with z3.
+               intro.
+               break_if; Zbool_to_Prop; try lia; auto.
+               Zbool_to_Prop.
+               lia.
+               simpl in Heqp0.
+               erewrite Heqp0.
+               easy.
+               (* bounds *)
+               admit.
+               admit.
+               }
+             erewrite N.
+             admit. } *)
+                 forward.
+                 admit. (* entailer! *)
+                 admit. (* entailer! *)
+                 discriminate.
+                **** (* ADVANCE *)
+                 match goal with
+                 | [ _ : _ |- semax _ ?Pre ?C ?Post ] =>
+                   forward_empty_while_break 
+                     (PROP (0 < z0; 0 < z2; 0 < z3; z0 <> 0; z2 <> -1;
+                            z2 <> 0; z1 = nth 0 (tags td) 0)
+  LOCAL (temp _consumed_myself (Vint (Int.repr 0 + (Int.repr z0 + Int.repr z2))%int);
+  temp _size (Vint (Int.repr size - (Int.repr z0 + Int.repr z2))%int);
+  temp _ptr
+    (Vptr b
+       (i +
+        Ptrofs.repr (sizeof tschar) * 
+        ptrofs_of_int Unsigned (Int.repr z0 + Int.repr z2)%int)%ptrofs);
+  temp _num__2 (Vint (Int.repr z0 + Int.repr z2)%int);
+  temp _limit_len
+    (Vint
+       (Int.repr
+          (Byte.unsigned
+             (Byte.repr
+                (snd
+                   (Exec.ber_fetch_len (sublist 1 (len ptr) ptr) 0 0 
+                      (size - z0) (sizeof tuint) Int.modulus)))) + 
+        Int.repr z0 + Int.repr z2)%int);
+  temp _t'29
+    (Vubyte
+       (Byte.repr
+          (snd
+             (Exec.ber_fetch_len (sublist 1 (len ptr) ptr) 0 0 (size - z0) 
+                (sizeof tuint) Int.modulus)))); 
+  temp _len_len (Vint (Int.repr z2));
+  temp _t'30 (Vint (Int.repr (len (tags td)))); 
+  temp _t'15 Vzero; 
+  temp _tlv_constr (Vint 0%int);
+  temp _t'13 Vzero; temp _t'34 (Znth 0 (map Vint (map Int.repr ptr)));
+  temp _tag_len (Vint (Int.repr z0)); temp _t'35 (Vint (Int.repr (len (tags td))));
+  temp _t'10 (Val.of_bool (Int.repr 0 == Int.repr (len (tags td)))%int);
+  temp _tagno (Vint (Int.repr z)); temp _t'4 Vzero; 
+  temp _t'3 (Vint (Int.repr 0));
+  temp _step (Vint (Int.repr z)); temp _t'1 Vzero;
+  temp _expect_00_terminators (Vint (Int.repr 0));
+  lvar _rval__12 (Tstruct _asn_dec_rval_s noattr) v_rval__12;
+  lvar _rval__11 (Tstruct _asn_dec_rval_s noattr) v_rval__11;
+  lvar _rval__10 (Tstruct _asn_dec_rval_s noattr) v_rval__10;
+  lvar _rval__9 (Tstruct _asn_dec_rval_s noattr) v_rval__9;
+  lvar _rval__8 (Tstruct _asn_dec_rval_s noattr) v_rval__8;
+  lvar _rval__7 (Tstruct _asn_dec_rval_s noattr) v_rval__7;
+  lvar _rval__6 (Tstruct _asn_dec_rval_s noattr) v_rval__6;
+  lvar _rval__5 (Tstruct _asn_dec_rval_s noattr) v_rval__5;
+  lvar _rval__4 (Tstruct _asn_dec_rval_s noattr) v_rval__4;
+  lvar _rval__3 (Tstruct _asn_dec_rval_s noattr) v_rval__3;
+  lvar _rval__2 (Tstruct _asn_dec_rval_s noattr) v_rval__2;
+  lvar _rval__1 (Tstruct _asn_dec_rval_s noattr) v_rval__1;
+  lvar _rval (Tstruct _asn_dec_rval_s noattr) v_rval; lvar _tlv_len tint v_tlv_len;
+  lvar _tlv_tag tuint v_tlv_tag; temp __res res_p; temp _opt_codec_ctx opt_codec_ctx_p;
+  temp _td td_p; temp _opt_ctx nullval; temp _tag_mode (Vint (Int.repr 0));
+  temp _last_tag_form (Vint (Int.repr 0)); temp _last_length last_length_p;
+  temp _opt_tlv_form nullval)
+  SEP (data_at Tsh (tarray tuchar (len (sublist 1 (len ptr) ptr)))
+         (map Vubyte (map Byte.repr (sublist 1 (len ptr) ptr)))
+         (Vptr b (i + Ptrofs.repr z0)%ptrofs);
+  data_at Tsh tint
+    (Vubyte
+       (Byte.repr
+          (snd
+             (Exec.ber_fetch_len (sublist 1 (len ptr) ptr) 0 0 (size - z0) 
+                (sizeof tuint) Int.modulus)))) v_tlv_len;
+  data_at Tsh tuchar (Vubyte (Byte.repr (Znth 0 ptr))) (Vptr b i);
+  data_at Tsh tuint (Vubyte (Byte.repr (snd (Exec.ber_fetch_tags ptr size 0 (sizeof tuint)))))
+    v_tlv_tag;
+  data_at Tsh (Tstruct _asn_codec_ctx_s noattr) (Vint (Int.repr max_stack_size)) opt_codec_ctx_p;
+  data_at_ Tsh (Tstruct _asn_dec_rval_s noattr) v_rval__12;
+  data_at_ Tsh (Tstruct _asn_dec_rval_s noattr) v_rval__11;
+  data_at_ Tsh (Tstruct _asn_dec_rval_s noattr) v_rval__10;
+  data_at_ Tsh (Tstruct _asn_dec_rval_s noattr) v_rval__9;
+  data_at_ Tsh (Tstruct _asn_dec_rval_s noattr) v_rval__8;
+  data_at_ Tsh (Tstruct _asn_dec_rval_s noattr) v_rval__7;
+  data_at_ Tsh (Tstruct _asn_dec_rval_s noattr) v_rval__6;
+  data_at_ Tsh (Tstruct _asn_dec_rval_s noattr) v_rval__5;
+  data_at_ Tsh (Tstruct _asn_dec_rval_s noattr) v_rval__4;
+  data_at_ Tsh (Tstruct _asn_dec_rval_s noattr) v_rval__3;
+  data_at_ Tsh (Tstruct _asn_dec_rval_s noattr) v_rval__2;
+  data_at_ Tsh (Tstruct _asn_dec_rval_s noattr) v_rval__1;
+  data_at_ Tsh (Tstruct _asn_dec_rval_s noattr) v_rval;
+  field_at Tsh (Tstruct _asn_TYPE_descriptor_s noattr) (DOT _tags) tags_p td_p;
+  field_at Tsh (Tstruct _asn_TYPE_descriptor_s noattr) (DOT _tags_count)
+    (Vint (Int.repr (len (tags td)))) td_p;
+  data_at Tsh (tarray tuint (len (tags td))) (map Vint (map Int.repr (tags td))) tags_p;
+  data_at_ Tsh asn_dec_rval_s res_p; data_at_ Tsh tint last_length_p))
+                 end.
+                 admit.
+                 repeat forward.
+                 admit. (* entailer!. *)
+                 admit.
+                 forward_if.
+                 ***** 
+                   (* z3 < size - z0 - z2 *) 
+                 forward.
+                 entailer!.
+                 repeat split; do 2 f_equal.
+                 rewrite Byte.unsigned_repr.
+                 erewrite Heqp0.
+                 cbn.
+                 lia.
+                 assert (ber_fetch_len_bounds :
+                           forall (ptr : list Z) (isc len_r size sizeofval rssizem : Z),
+                          0 <=  len_r <= 255 ->
+                         Forall (fun x => 0 <= x <= Byte.max_unsigned) ptr ->
+                         snd (Exec.ber_fetch_len ptr isc len_r size sizeofval rssizem) <> -1 ->
+                        0 <= snd (Exec.ber_fetch_len ptr isc len_r size sizeofval rssizem) 
+                        <= Byte.max_unsigned).
+                 { intros.
+                   unfold Exec.ber_fetch_len in H46.
+                    unfold Exec.ber_fetch_len.
+                   repeat break_if; cbn; try lia.
+                   admit.
+                   admit.
+                   repeat break_let.
+                   admit. }
+                 eapply ber_fetch_len_bounds.
+                 lia.
+                 (* add to PRE:
+                   Forall (fun x : Z => 0 <= x <= Byte.max_unsigned) ptr
+                  also precondition to fetch length *)
+                 admit.
+                 
+                 eapply repr_neq_e in H11.
+                 generalize H11.
+                 rewrite Byte.unsigned_repr.
+                 easy.
+                 admit.
+                 cbn.
+                 f_equal.
+                 strip_repr.
+                 (* NEED: 0 <= z0 + z2 <= Int.max_unsigned *)
+                 admit.
+                 replace (size - z0 - z2 >? z3) with true. 
+                  (* true  *)
+                 admit.
+                   (* true  *)
+                 symmetry.
+                 generalize H17.
+                 rewrite Byte.unsigned_repr.
+                 simpl in Heqp0.
+                 erewrite Heqp0.
+                 strip_repr.
+                 intro.
+                 erewrite Z.gtb_lt.
+                 lia.
+                 (* Int.min_signed <= size - (z0 + z2) <= Int.max_signed *)
+                 admit.
+                 admit.
+                 erewrite Heqp0.
+                 erewrite Heqp.
+                 simpl.
+                 entailer!.
+                 admit.
+                 (* check Bytes and Int *)
+                 *****
+                 forward.
+                 entailer!.
+                 repeat split; do 2 f_equal.
+                 (* true *)
+                 admit.
+                 (* true *)
+                 admit.
+                 replace (size - z0 - z2 >? z3)  with false by admit.
+                 lia.
+                 (* true  *)
+                 admit.
+                 (* true  *)
+                 
+                **** admit.
+                **** admit.
+               *** admit.
+           * Zbool_to_Prop.
+              simpl.
+             Intros.
+             Zbool_to_Prop.
+             forward.
+           forward_if.
+           generalize H3.
+           strip_repr.
+           intro.
+           lia.
+         (*  unfold POSTCONDITION.
+           unfold abbreviate.
+           simpl. *)
+           forward.
+           assert (z = 1) as Z by lia.
+           erewrite Z.
+           entailer!.
+           (* do 2 f_equal. try lia. *)
+      +++  (* CONTINUE  to LI *)
+          repeat break_let.
+          forward.
+          forward.
+          Exists 1.
+          repeat rewrite_if_b.
+          repeat break_let.
+          entailer!.
+          break_if; Zbool_to_Prop; try lia.
+          break_if; Zbool_to_Prop; try lia.          
+          entailer!.         
+      +++ (* BREAK to rest *)
+          repeat break_let.
+          forward_if True; try contradiction.
+          forward.
+          entailer!.
+          
+          forward_if_add_sep (data_at Tsh tint (Vint (Int.repr z2)) last_length_p) 
+                             last_length_p; try contradiction.
+          forward.
+          forward.
+          entailer!.
+          (* RETURN OK *)
+          forward_empty_while.
+          forward_if True; try contradiction.
+          forward.
+          entailer!.
+          forward_if (temp _t'25 Vone); try contradiction.
+          forward.
+          entailer!.
+          discriminate.
+          forward_if_add_sep
+            (data_at Tsh (Tstruct _asn_dec_rval_s noattr)
+                     (Vint (Int.repr 0), (Vint (Int.repr (z + z1))))
+                     v_rval__12) v_rval__12. 
+          forward.
+          entailer!. 
+          discriminate.
+          repeat forward.
+          assert (ber_check_tags_primitive
+                    ptr td max_stack_size size (sizeof tuint)
+                    Int.modulus = Some (z2, z + z1)) as B.
+          {  unfold ber_check_tags_primitive.             
+             erewrite Heqp.
+             erewrite Heqp0.
+             repeat rewrite_if_b.            
+             repeat break_if;
+               try destruct_orb_hyp;
+               repeat rewrite_if_b; symmetry; repeat Zbool_to_Prop;
+                 try lia; auto. }
+          erewrite B.
+          entailer!.
+Admitted.
+*)
+End Ber_check_tags.
